Deletion of unnecessary files and renaming

proof/absspec/XMSS_Security_RFCAbs.ec
@@ -1,4 +1,4 @@
-require import AllCore IntDiv List StdOrder RealExp Distr DList.
+require import AllCore IntDiv List Distr DList StdOrder RealExp.
 require import BitEncoding.
 (*---*) import BitChunking.
 
@@ -7,22 +7,197 @@ require import Array8.
 
 require (****) XMSS_TW.
 require import XMSS_RFC_Abs.
-import XMSS_RFC_Params Address BaseW.
-
+import XMSS_RFC_Params WOTS Address BaseW.
+(*
+require (****) XMSS_TW.
+require import XMSS_PRF.
+import Params Types XMSS_Types Hash WOTS Address LTree BaseW.
+*)
 import IntOrder.
+
+(* Overflows may happen unless h is upper bounded *)
+axiom h_max : h < 32.
+
+(* We are using multiples of n and len to distinguish which hash to use *)
+axiom gt0_n : 0 < n.
+
 
 op BitsToBytes (bits : bool list) : W8.t list = map W8.bits2w (chunk W8.size bits).
 op BytesToBits (bytes : W8.t list) : bool list = flatten (map W8.w2bits bytes).
+
+lemma BitsToBytesK x : 8 %| size x => BytesToBits (BitsToBytes x) = x.
+move => Hx.
+rewrite /BitsToBytes /BytesToBits.
+rewrite -map_comp /(\o) /=.
+have [H _]:= (eq_in_map (fun (x0 : bool list) => w2bits (W8.bits2w x0)) idfun (chunk 8 x)).
+rewrite H;1: by move => x0 memX0 /=; rewrite W8.bits2wK; smt(in_chunk_size).
+rewrite map_id chunkK //.
+qed.
+
+lemma BytesToBitsK x : (BitsToBytes (BytesToBits x)) = x.
+rewrite /BitsToBytes /BytesToBits.
+rewrite flattenK;1,2: smt(mapP W8.size_w2bits).
+rewrite -map_comp /(\o).
+have [H _]:= (eq_in_map (fun (x0 : W8.t) => W8.bits2w (W8.w2bits x0)) idfun x).
+rewrite H;1: by move => x0 memX0 /=.
+by smt(map_id).
+qed.
+
 op W64toBytes_ext (x : W64.t) (l : int) : W8.t list =
   rev (mkseq (fun i => nth W8.zero (to_list (W8u8.unpack8 x)) i) l).
 
-op idxs2adrs (il : int list) : adrs =
+(*
+  Conversion operators
+  --------------------
+  Security spec indices (corresponding to an address):
+    [hash    | padding(= 0) | tree breadth;
+     chain   | padding(= 0) | tree height;
+     keypair | keypair      | padding(= 0);
+     chtype  | pkcotype     | trhtype]
+  RFC address:
+    [layer(= 0);
+     hypertree1(= 0);
+     hypertree2(= 0);
+     chtype(= 0) | ltrtype(= 1)  | trhtype(= 2);
+     keypair     | keypair       | padding(= 0);
+     chain       | tree height   | tree height;
+     hash        | tree breadth  | tree breadth;
+     keyAndMask]
+
+  If we have set the abstraction (of the hash functions) up properly, we only need
+  to consider parts of the addresses that (conceptually) overlap between the two.
+  Particularly:
+  - The layer, hypertree1, hypertree2 are always 0 on the RFC side, as we are dealing with single-tree XMSS,
+    making them irrelevant.
+  - The tree height and tree breadth indices used for ltree/public key compression on the RFC side
+    are abstracted away under the relevant hash function (security: pkco, RFC: ltree).
+    Specifically, these indices are also always 0 as far as we can tell here (and their usage/manipulation
+    is done "inside the hash functions").
+  - The keyAndMask index on the RFC side is also abstracted away under the relevant hash functions.
+    (Indeed,  this index is also always 0 as far as we can tell here, and its usage/manipulation
+    is done "inside the hash functions").
+*)
+(* Indices of security spec -> address in implementation/RFC *)
+op idxs2adr (il : int list) : adrs =
   init (fun (i : int) =>
         if 3 <= i <= 6
         then W32.of_int (nth witness il (6 - i))
         else W32.zero).
 
-clone XMSS_TW as XMSS_Security with
+(* Address in implementation/RFC -> Indices of security spec *)
+op adr2idxs (ad : Address.adrs) : int list =
+  rev (map W32.to_uint (sub ad 3 4)).
+
+lemma idxs2adrK (il : int list) :
+  size il = 4 =>
+  all (mem (range 0 W32.modulus)) il =>
+  adr2idxs (idxs2adr il) = il.
+proof.
+move=> eq4szil mem_il.
+have eq4szm : size (adr2idxs (idxs2adr il)) = 4.
++ by rewrite size_rev size_map size_mkseq.
+rewrite &(eq_from_nth witness) eq4szm 1:eq4szil // => i rngi.
+rewrite /adr2idxs nth_rev size_map size_sub 1..3://.
+rewrite (nth_map witness witness) 1:size_sub 1:// 1:/#.
+rewrite nth_mkseq 1:/# /= /idxs2adr initiE 1:/# /= (: 3 <= 7 - (i + 1) <= 6) 1:/# /=.
+rewrite of_uintK pmod_small 2:/#.
+by move/(all_nthP _ _ witness): mem_il => /(_ i _); smt(mem_range).
+qed.
+
+lemma adr2idxsK (ad : Address.adrs) :
+  (forall i, 0 <= i < 3 \/ i = 7 => ad.[i] = W32.zero) =>
+  idxs2adr (adr2idxs ad) = ad.
+proof.
+move=> zr.
+rewrite /adr2idxs /idxs2adr tP => i rngi.
+rewrite initE rngi /=; case (0 <= i < 3 \/ i = 7) => outi.
++ by move: (zr i outi) => -> /#.
+rewrite ifT 1:/# nth_rev 2:(nth_map witness); 1,2:smt(size_map size_sub).
+by rewrite to_uintK nth_sub; smt(size_sub size_map).
+qed.
+
+
+(*
+lemma adr2idxsK (ad : Address.adrs) :
+
+  idxs2adr (adr2idxs ad) = ad.
+proof.
+*)
+(* Get checksum from XMSS_Checksum and then plug those results
+   here
+- Make space in detailed chapters for discussion in introduction
+  > what do difficulties reveal about actual crypto
+  > clear explanation of things that want to make a point about that are relevant
+    to crypto:
+      Delaying of delaying key gen, requireing that it is stateless
+      SSP: explain enough of
+
+-
+
+
+clone import XMSS_TW as XMSS_ABSTRACT with
+  type mseed <- nbytes,
+  op dmseed <- (dmap ((dlist W8.dword Params.n)) NBytes.insubd),
+  type mkey <- nbytes * int,
+  type msgXMSSTW <- W8.t list,
+  type FLXMSSTW.SA.WTW.pseed <- nbytes,
+  op FLXMSSTW.SA.WTW.dpseed <- (dmap ((dlist W8.dword n)) NBytes.insubd),
+  type FLXMSSTW.SA.WTW.sseed <- nbytes,
+  op FLXMSSTW.SA.WTW.dsseed <- (dmap ((dlist W8.dword n)) NBytes.insubd),
+  type FLXMSSTW.SA.HAX.Adrs.sT <- adrs,
+  op FLXMSSTW.n <- n,
+  op FLXMSSTW.h <- h,
+  op FLXMSSTW.log2_w <- ilog 2 w,
+  op FLXMSSTW.chtype <= 0,
+  op FLXMSSTW.pkcotype <= 1,
+  op FLXMSSTW.trhtype <= 2,
+  op mkg = (fun (ms : nbytes) (i : FLXMSSTW.SA.index) =>
+        let padding =  W64toBytes_ext prf_padding_val padding_len in
+        let in_0 = toByte (W32.of_int (FLXMSSTW.SA.Index.val i)) 4 in
+        (Hash (padding ++ NBytes.val ms ++ in_0), FLXMSSTW.SA.Index.val i)),
+  op FLXMSSTW.SA.WTW.prf_sk =
+    (fun (ss : nbytes) (psad : nbytes * adrs) =>
+     let adbytes = addr_to_bytes (set_key_and_mask psad.`2 0) in
+     (DigestBlock.insubd
+      (BytesToBits
+       (NBytes.val
+        (prf_keygen (NBytes.val psad.`1 ++ NBytes.val adbytes) ss))))),
+  op FLXMSSTW.SA.WTW.thfc =
+    (fun (i : int) (ps : nbytes) (ad : adrs) (x : bool list) =>
+     if i = 8 * n then
+      (let adbytes0 = addr_to_bytes (set_key_and_mask ad 0) in
+       let k = prf adbytes0 ps in
+       let adbytes1 = addr_to_bytes (set_key_and_mask ad 1) in
+       let bitmask = prf adbytes1 ps in
+       (DigestBlock.insubd
+        (BytesToBits
+         (NBytes.val
+          (_F k (NBytes.insubd (bytexor (BitsToBytes x) (NBytes.val bitmask))))))))
+     else if i = 8 * n * 2 then
+      (let xw = BitsToBytes x in
+       let l = take (size xw %/ 2) xw in
+       let r = drop (size xw %/ 2) xw in
+       (DigestBlock.insubd
+        (BytesToBits
+         (NBytes.val
+          (rand_hash (NBytes.insubd l) (NBytes.insubd r) ps ad)))))
+     else if i = 8 * n * len then
+      (let wpk = LenNBytes.insubd (map NBytes.insubd (chunk n (BitsToBytes x))) in
+       (DigestBlock.insubd
+        (BytesToBits
+         (NBytes.val
+          (ltree ps ad wpk)))))
+     else witness)
+proof FLXMSSTW.val_log2w, FLXMSSTW.dist_adrstypes.
+realize FLXMSSTW.val_log2w.
+case: w_vals => ->; [left | right; left].
++ by rewrite (: 4 = 2 ^ 2).
+by rewrite (: 16 = 2 ^ 4).
+qed.
+realize FLXMSSTW.dist_adrstypes by trivial.
+*)
+
+clone import XMSS_TW as XMSS_Security with
   type mseed <- nbytes,
   type mkey <- nbytes,
   type msgXMSSTW <- W8.t list,
@@ -30,34 +205,37 @@ clone XMSS_TW as XMSS_Security with
     (fun (ms : nbytes) (i : FLXMSSTW.SA.index) =>
      prf ms (NBytes.insubd (toByte (W32.of_int (FLXMSSTW.SA.Index.val i)) n))),
   op dmseed <- dmap (dlist W8.dword Params.n) NBytes.insubd,
-  (* TODO: op MKey.enum <- map NBytes.insubd <all W8.t lists of length n>
-  op dmkey <- duniform MKey.enum, *)
+  op MKey.enum <= map NBytes.insubd (mkseq (fun (i : int) => BitsToBytes (BS2Int.int2bs (8 * n) i)) (2 ^ (8 * n))),
+  op dmkey <- duniform MKey.enum,
   op FLXMSSTW.n <- n,
   op FLXMSSTW.log2_w <- ilog 2 w,
   op FLXMSSTW.h <- h,
   op FLXMSSTW.chtype <= 0,
   op FLXMSSTW.pkcotype <= 1,
   op FLXMSSTW.trhtype <= 2,
+  op FLXMSSTW.SA.adc <= FLXMSSTW.SA.XAddress.insubd (FLXMSSTW.SA.HAX.Adrs.insubd
+                                                     (adr2idxs (zero_address))),
   op FLXMSSTW.SA.dmsgFLXMSSTW <- duniform FLXMSSTW.SA.WTW.DigestBlockFT.enum,
   type FLXMSSTW.SA.WTW.pseed <- nbytes,
   type FLXMSSTW.SA.WTW.sseed <- nbytes,
   op FLXMSSTW.SA.WTW.dsseed <- dmap (dlist W8.dword Params.n) NBytes.insubd,
   op FLXMSSTW.SA.WTW.dpseed <- dmap (dlist W8.dword Params.n) NBytes.insubd,
+  op FLXMSSTW.SA.WTW.ddgstblock <- duniform FLXMSSTW.SA.WTW.DigestBlockFT.enum,
   op FLXMSSTW.SA.WTW.prf_sk <-
     (fun (ss : nbytes) (psad : nbytes * FLXMSSTW.SA.adrs) =>
      DigestBlock.insubd (BytesToBits
                          (NBytes.val
-                          (WOTS.prf_keygen ss (psad.`1, (idxs2adrs (FLXMSSTW.SA.HAX.Adrs.val psad.`2))))))),
+                          (prf_keygen ss (psad.`1, (idxs2adr (FLXMSSTW.SA.HAX.Adrs.val psad.`2))))))),
   op FLXMSSTW.SA.WTW.thfc <-
     (fun (i : int) (ps : nbytes) (ad : FLXMSSTW.SA.adrs) (x : bool list) =>
      let nb2db = (fun (x : nbytes) => DigestBlock.insubd (BytesToBits (NBytes.val x))) in
-     let mad = (idxs2adrs (FLXMSSTW.SA.HAX.Adrs.val ad)) in
+     let mad = (idxs2adr (FLXMSSTW.SA.HAX.Adrs.val ad)) in
      if i = 8 * n then
-      nb2db (WOTS.f ps mad (NBytes.insubd (BitsToBytes x)))
+      nb2db (f ps mad (NBytes.insubd (BitsToBytes x)))
      else if i = 8 * n * 2 then
       let xl = take (8 * n) x in
       let xr = drop (8 * n) x in
-      nb2db (rand_hash ps mad (NBytes.insubd (BitsToBytes xl)) (NBytes.insubd (BitsToBytes xl)))
+      nb2db (rand_hash ps mad (NBytes.insubd (BitsToBytes xl)) (NBytes.insubd (BitsToBytes xr)))
      else if i = 8 * n * len then
       let wpk = LenNBytes.insubd (map NBytes.insubd (chunk n (BitsToBytes x))) in
       nb2db (ltree ps mad wpk)
@@ -79,12 +257,2716 @@ realize FLXMSSTW.SA.dmsgFLXMSSTW_uni by exact: duniform_uni.
 realize FLXMSSTW.SA.dmsgFLXMSSTW_fu by apply /duniform_fu /WTW.DigestBlockFT.enumP.
 realize FLXMSSTW.SA.WTW.dsseed_ll by apply /dmap_ll /dlist_ll /W8.dword_ll.
 realize FLXMSSTW.SA.WTW.dpseed_ll by apply /dmap_ll /dlist_ll /W8.dword_ll.
-realize FLXMSSTW.SA.WTW.ddgstblock_ll. admitted. (* TODO: Proof artifact, not needed (might instantiate just because?) *)
-realize MKey.enum_spec. admitted. (* TODO: instantiate enum and prove, but shouldn't be necessary *)
+realize FLXMSSTW.SA.WTW.ddgstblock_ll.
+rewrite duniform_ll -size_eq0 2!size_map size_range.
+suff /#: 0 < 2 ^ (8 * n).
+by rewrite expr_gt0.
+qed.
+realize MKey.enum_spec.
+move => x; rewrite count_uniq_mem.
++ rewrite ?map_inj_in_uniq /= 3:iota_uniq.
+  + move=> xl yl /mapP [x' /= [xpin ->]] /mapP [y' /= [ypin ->]] eqins.
+    rewrite -NBytes.insubdK 2:eq_sym 2:-NBytes.insubdK 3:eqins //.
+    + rewrite /BitsToBytes size_map size_chunk 1:// BS2Int.size_int2bs.
+      by rewrite lez_maxr 2:mulKz 2://; 1:smt(ge1_n).
+    rewrite /BitsToBytes size_map size_chunk 1:// BS2Int.size_int2bs.
+    by rewrite lez_maxr 2:mulKz 2://; 1:smt(ge1_n).
+  move=> x' y' /mem_iota /= rng_x /mem_iota /= rng_y eqb2b.
+  suff eqbs: (BS2Int.int2bs (8 * n) x') = (BS2Int.int2bs (8 * n) y').
+  +  by rewrite -(BS2Int.int2bsK (8 * n)) 3:eq_sym 3:-(BS2Int.int2bsK (8 * n)); smt(ge1_n).
+  rewrite -BitsToBytesK; 1: by rewrite BS2Int.size_int2bs lez_maxr 2:dvdz_mulr; 1: smt(ge1_n).
+  by rewrite eq_sym -BitsToBytesK; 1: rewrite BS2Int.size_int2bs lez_maxr 2:dvdz_mulr; smt(ge1_n).
+rewrite /b2i mapP ifT 2://; 1: exists (NBytes.val x).
+rewrite NBytes.valKd /= mapP; exists (BS2Int.bs2int (BytesToBits (NBytes.val x))).
+rewrite /= (: 8 * n = size (BytesToBits (NBytes.val x))).
++ rewrite /BytesToBits (size_flatten_ctt 8).
+  + by move=> bs /mapP [x' ->]; rewrite size_w2bits.
+  by congr; rewrite size_map NBytes.valP.
+by rewrite BS2Int.bs2intK BytesToBitsK mem_iota BS2Int.bs2int_ge0 BS2Int.bs2int_le2Xs.
+qed.
 realize MsgXMSSTW.enum_spec. admitted. (* TODO: this shouldn't be necessary *)
-realize rng_qS. admitted. (* TODO: Proof artifact, move to section *)
-realize ge0_qH. admitted. (* TODO: Proof artifact, move to section *)
 realize dmseed_ll by apply /dmap_ll /dlist_ll /W8.dword_ll.
-realize dmkey_ll. admitted. (* TODO: instantiate and can do *)
-realize dmkey_uni. admitted. (* TODO: instantiate and can do *)
-realize dmkey_fu. admitted. (* TODO: instantiate and can do *)
+realize dmkey_ll.
+rewrite duniform_ll -size_eq0 2!size_map size_iota.
+suff /#: 0 < 2 ^ (8 * n).
+by rewrite expr_gt0.
+qed.
+realize dmkey_uni by exact: duniform_uni.
+realize dmkey_fu by apply /duniform_fu /MKey.enumP.
+
+import RFC HtSRFC Repro MCORO.
+import FLXMSSTW SA WTW.
+
+lemma gt2_len : 2 < XMSS_Security.FLXMSSTW.len.
+proof.
+rewrite /len /len1 /len2 /= /len1 /len2 /w /w.
+admitted.
+
+
+lemma l_max : l < 4294967296
+  by rewrite -pow2_32 /l;apply gt_exprsbde; smt(h_g0 h_max).
+
+
+op bs2block(a : nbytes) = DigestBlock.insubd (BytesToBits (NBytes.val a)).
+op block2bs(a : dgstblock): nbytes = NBytes.insubd (BitsToBytes (DigestBlock.val a)).
+op ads2adr (ad : SA.adrs) : Address.adrs = idxs2adr (HAX.Adrs.val ad).
+op adr2ads (ad : Address.adrs) : SA.adrs = HAX.Adrs.insubd (adr2idxs ad).
+
+lemma ads2adrK (ad : SA.adrs) :
+  all (mem (range 0 W32.modulus)) (HAX.Adrs.val ad) =>
+  adr2ads (ads2adr ad) = ad.
+proof. move=> *; smt(HAX.Adrs.valP HAX.Adrs.valKd idxs2adrK). qed.
+
+lemma adr2adsK (ad : Address.adrs) :
+  (forall i, 0 <= i < 3 \/ i = 7 => ad.[i] = W32.zero) =>
+  valid_adrsidxs (adr2idxs ad) =>
+  ads2adr (adr2ads ad) = ad.
+proof. smt(HAX.Adrs.insubdK adr2idxsK). qed.
+
+(* Notes:
+- We have a full binary tree with  h+1 levels (height = h), so 2^h leaves
+  (and 2^(h + 1) - 1 total nodes, i.e., leaves and inner nodes combined).
+- Levels are indexed from bottom to top, leaves at level 0, root at level h
+- The length of a full path to a leaf is h
+- The length of the path to a node at level l \in [0..h] is h - l (root path is [])
+- The path to a leaf can be extracted from the bit representation of its index:
+    the i-th leaf can be found at path rev (bits h i)
+- throughout we will need the corner case of the leaf with index 2^h when
+  we exit the loop, where everything works in a tree of height h+1
+*)
+
+type path = bool list.
+
+(* The hamming weight of a path determines the size of the stack *)
+op hw (p : path) = count (pred1 true) p.
+
+(* The path of a leaf; we need the corner case of leaf 2^h for exiting the loop *)
+op lpath (lidx : int) =
+  rev (BS2Int.int2bs (h + (b2i (lidx = 2^h))) lidx).
+
+lemma size_lpath (lidx : int) :
+  0 <= lidx <= 2^h => size (lpath lidx) = if lidx = 2^h then (h+1) else h.
+proof.
+by move=> hle @/lpath; rewrite size_rev BS2Int.size_int2bs; smt(h_g0).
+qed.
+
+lemma size_lpath_lt (lidx : int) :
+  0 <= lidx < 2^h => size (lpath lidx) = h.
+proof. by move=> ?; rewrite size_lpath /#. qed.
+
+(* When working in subtrees of height t we need the suffix of length t
+   of the path to the leaf, except in the corner case where we are at
+   the end.  *)
+op  prefix(s : 'a list, t : int) = take (size s - t) s.
+op  suffix(s : 'a list, t : int) = drop (size s - t) s.
+
+(* The path of the exit leaf is not a prefix of the path
+   in the full tree, but it makes the theorems nicely commute *)
+op lpathst (lidxo t : int) = 
+  rev (BS2Int.int2bs (t + (b2i (lidxo = 2^t))) lidxo).
+
+(* Exiting a subtree breaks this identity *)
+lemma lpathst_suffix (start lidxo t : int) :
+   0 <= start <= 2^h - 2^t
+=> 0 <= t <= h
+=> 0 <= lidxo < 2^t
+ => 2^t %| start
+=> lpathst lidxo t =  suffix (lpath (start + lidxo)) t.
+move => *. 
+rewrite /lpathst /lpath /suffix size_rev BS2Int.size_int2bs /=.
+have -> /= : b2i (lidxo = 2 ^ t) = 0 by smt().
+have -> /= : b2i (start + lidxo = 2 ^ h) = 0 by smt().
+have -> /= : (max 0 h - t) = h-t by smt().
+have -> := BS2Int.int2bs_cat t h (start + lidxo) _;1:smt().
+rewrite rev_cat drop_cat_le ifT; 1: smt(size_take size_rev BS2Int.size_int2bs h_g0).
+rewrite drop_oversize /=;1: smt(size_take size_rev BS2Int.size_int2bs h_g0).
+congr;apply BS2Int.bs2int_eq;1,2:smt().
+smt().
+qed.
+
+lemma size_lpathst (lidxo t : int) :
+   0 <= t <= h
+=> 0 <= lidxo <= 2^t
+=> size (lpathst lidxo t) = if lidxo = 2^t then (t+1) else t.
+proof.
+move=> ?? @/lpathst;rewrite size_rev BS2Int.size_int2bs; smt().
+qed.
+
+lemma size_lpathst_lt (lidxo t : int) :
+   0 <= t <= h
+=> 0 <= lidxo < 2^t
+=> size (lpathst lidxo t) = t.
+proof. by move=> *; rewrite size_lpathst /#. qed.
+
+(*
+                     +
+               +           +
+           +      +     +     +
+          0 1    2 3   4 5   6 7
+
+path to 5 = 1 0 1 => stack contains [0] and [1 0 0]
+path to 6 = 1 1 0 => stack contains [0] and [1 0]
+
+*)
+
+(* The paths of all the sibling nodes of 1-bit choices in a leaf path *)
+op extract_path (p : path) (i : int) =
+  if   nth false p i
+  then Some (rcons (take i p) false)
+  else None.
+
+op paths_from_leaf ( lidxo t : int) : path list =
+  if (lidxo = 2^t) then [[]] (* we get the root *) else
+  pmap (extract_path (lpathst lidxo t)) (range 0 t).
+
+(* Move to List *)
+lemma count_eq_nth ['a] (p : 'a -> bool) (s1 s2 : 'a list) :
+     size s1 = size s2
+  => (forall k, 0 <= k < size s1 => p (nth witness s1 k) = p (nth witness s2 k))
+  => count p s1 = count p s2.
+proof.
+elim: s1 s2 => [|x1 s1 ih] [|x2 s2] //=; ~-1:smt(size_ge0).
+(* Only solved by Z3 4.12.4 *)
+move/addzI => eq_sz heqp; rewrite (heqp 0) ?(ih s2) => *; smt(size_ge0).
+qed.
+
+lemma paths_from_leaf_root t : paths_from_leaf (2^t) t = [[]].
+proof. by rewrite /paths_from_leaf //=. qed.
+
+hint simplify paths_from_leaf_root.
+
+lemma lpath_root : lpath (2 ^ h) = true :: nseq h false.
+proof.
+have h_g0 := h_g0; move=> @/lpath @/b2i /=.
+rewrite BS2Int.int2bs_pow2 ?mem_range 1:/# /=.
+by rewrite nseq0 rev_cat /= rev_nseq.
+qed.
+
+lemma lpathst_root t :
+   0 <= t <= h
+=> lpathst  (2 ^ t) t = true :: nseq t false.
+proof.
+move => ht;move=> @/lpathst @/b2i /=.
+rewrite BS2Int.int2bs_pow2 ?mem_range 1:/# /=.
+by rewrite nseq0 rev_cat /= rev_nseq.
+qed.
+
+hint simplify lpath_root (* , lpathst_root *).
+
+lemma size_pmap ['a 'b] (p : 'a -> 'b option) (s : 'a list) :
+  size (pmap p s) = count (fun x => is_some (p x)) s.
+proof. by elim: s => //= x s ih; case: (p x) => /=; rewrite ih. qed.
+
+lemma rev_iota i j : rev (iota_ i j) = map (fun k => (i + j) - (k + 1)) (iota_ 0 j).
+proof.
+elim/natind: j i => [j le0_j|j ge0_j ih] i; first by rewrite !iota0.
+rewrite iotaSr // iotaS // rev_rcons map_cons ih /=; split; first smt().
+by rewrite (iota_addl 1 0) -map_comp /(\o) /#.
+qed.
+
+lemma rev_mkseq ['a] (f : int -> 'a) (n : int) :
+  rev (mkseq f n) = mkseq (fun i => f (n - (i + 1))) n.
+proof. by rewrite /mkseq -map_rev rev_iota map_comp. qed.
+
+lemma lpath_intdivE (lidx : int) : 0 <= lidx < 2^h =>
+  lpath lidx = mkseq (fun i => (lidx %/ 2^(h - (i + 1))) %% 2 <> 0) h.
+proof.
+move=> rg @/lpath; rewrite [lidx = _]ltr_eqF 1:/# b2i0 /=.
+by rewrite /BS2Int.int2bs rev_mkseq.
+qed.
+
+lemma hw_lpathE (lidx : int) : 0 <= lidx < 2^h =>
+  hw (lpath lidx) = count (fun i => lidx %/ 2^(h - (i + 1)) %% 2 <> 0) (range 0 h).
+proof. by move=> hrg; rewrite lpath_intdivE // /hw count_map /#. qed.
+
+require import IntMin.
+
+hint simplify b2i0, b2i1.
+
+lemma b2i0_eq (b : bool) : !b => b2i b = 0.
+proof. by case: b. qed.
+
+lemma hw_rev (p : bool list) : hw (rev p) = hw p.
+proof. by rewrite /hw count_rev. qed.
+
+lemma hw_cat (p1 p2 : bool list) : hw (p1 ++ p2) = hw p1 + hw p2.
+proof. by rewrite /hw count_cat. qed.
+
+lemma hw_nil : hw [] = 0.
+proof. by done. qed.
+
+hint simplify hw_nil.
+
+lemma ge0_hw (p : path) : 0 <= hw p.
+proof. by apply: count_ge0. qed.
+
+lemma hw_cons (b : bool) (p : bool list) : hw (b :: p) = b2i b + hw p.
+proof. by rewrite /hw /pred1; case: b. qed.
+
+hint simplify hw_cons.
+
+lemma hw_rcons (p : bool list) (b : bool) : hw (rcons p b) = b2i b + hw p.
+proof. by rewrite -cats1 hw_cat /= addrC. qed.
+
+lemma hw_nseq (n : int) (b : bool) : 0 <= n => hw (nseq n b) = b2i b * n.
+proof. by move=> ge0_n @/hw; rewrite count_nseq /pred1 /=; case: b => //#. qed.
+
+lemma pfl_r_size (p : path) (n : int) : size p <= n =>
+  size (pmap (extract_path p) (range 0 n)) = hw p.
+proof.
+move=> ltsz; rewrite (range_cat (size p)); ~-1: smt(size_ge0).
+rewrite pmap_cat size_cat addrC [size _](_ : _ = 0) /=.
+- apply/size_eq0; rewrite pmap_map eq_in_filter_pred0 //.
+  move=> @/predC1 /= q /mapP[i]; rewrite mem_range.
+  case=> rgi -> @/extract_path /=; rewrite iffalse //.
+  by rewrite nth_default 1:/#.
+elim/last_ind: {n ltsz} p => //=.
+- by move=> @/extract_path /=; rewrite range_geq.
+move=> p b ih; rewrite hw_rcons size_rcons.
+rewrite rangeSr; first smt(size_ge0).
+rewrite -[rcons _ (size _)]cats1 pmap_cat size_cat /=.
+rewrite fun_if /= [if _ then _ else _](_ : _ = b2i b).
+- by rewrite /extract_path nth_rcons /=; case: b.
+rewrite addrC -ih !size_pmap; congr; apply eq_in_count.
+move=> x /mem_range [ge0_x ltx] /= @/extract_path.
+rewrite nth_rcons [if x < _ then _ else _]iftrue //=.
+by case: (nth false p x).
+qed.
+
+lemma pfl_r_size_min (p : path) (n : int) : 0 <= n =>
+  size (pmap (extract_path p) (range 0 n)) = hw (take n p).
+proof.
+move=> ge0_n; case: (size p <= n).
+- by move=> ?; rewrite take_oversize // &(pfl_r_size).
+move/ltzNge => ltn; rewrite -(pfl_r_size _ n).
+- by rewrite size_take //#.
+rewrite !size_pmap &(eq_in_count) /= => i /mem_range rgi.
+rewrite /extract_path nth_take ~-1://#.
+by rewrite ![is_some (if nth _ _ _ then _ else _)]fun_if.
+qed.
+
+
+lemma pfl_size (lidxo t : int) :
+    0 <= t <= h 
+ => 0 <= lidxo <= 2^t
+ => size (paths_from_leaf lidxo t) = hw (lpathst lidxo t).
+proof.
+move => ?.
+have ? := h_g0; case=> ge0_lidx /lez_eqVlt [->|lt].
+- by rewrite /hw /= lpathst_root 1:/# /= count_nseq iffalse //=.
+rewrite /paths_from_leaf [lidxo = _]ltr_eqF //=.
+rewrite &(pfl_r_size) /lpathst /suffix. 
+by rewrite size_rev BS2Int.size_int2bs lez_maxr //#.
+qed.
+
+lemma hw_le_size (p : path) : hw p <= size p.
+proof. by rewrite /hw &(count_size). qed.
+
+lemma take_cat' ['a] (n : int) (s1 s2 : 'a list) :
+  take n (s1 ++ s2) = take n s1 ++ (take (n - size s1)) s2.
+proof.
+rewrite take_cat; case: (n < size s1) => ?.
+- by rewrite [take (_ - _) _]take_le0 ?cats0 //#.
+- by rewrite [take n s1]take_oversize //#.
+qed.
+
+lemma pfl_eq (p1 p2 : path) (n k : int) :
+     0 <= n
+  => 0 <= k
+  => (forall n, 0 <= n => hw (take n p1) < k \/ hw (take n p2) < k => take (n+1) p1 = take (n+1) p2)
+  => k <= hw p1
+  => k <= hw p2
+  =>   take k (pmap (extract_path p1) (range 0 n))
+     = take k (pmap (extract_path p2) (range 0 n)).
+proof.
+move=> ge0_n ge0_k eq hw1 hw2; elim: n ge0_n => /= [|n ge0_n ih].
+- by rewrite range_geq.
+rewrite !rangeSr // -cats1 !pmap_cat /= !take_cat'.
+rewrite !pfl_r_size_min // -ih; congr.
+case: (hw (take n p1) < k \/ hw (take n p2) < k) => cmp; last first.
+- by rewrite ![take (k - _) _]take_le0 //#.
+have {eq}eq := eq n ge0_n cmp.
+have <-: take n p1 = take n p2.
+- by move/(congr1 (take n)): eq; rewrite !take_take iftrue //#.
+suff <-: extract_path p1 n = extract_path p2 n by done.
+rewrite /extract_path; congr.
+- move/(congr1 (fun s => nth false s n)): eq => /=.
+  by rewrite !nth_take ~-1://#.
+- by move/(congr1 (take n)): eq; rewrite !take_take iftrue //#.
+qed.
+
+(* The list of leaves that are under a node given by a path *)
+op leaves_from_path (p : path) =
+ if 0 <= size p <= h then
+    let hsub = h - size p in
+    mkseq (fun i => BS2Int.bs2int (rev p) * 2^hsub + i) (2^hsub)
+ else witness.
+
+lemma lfp_leaf lidx : 0 <= lidx < 2^h => (leaves_from_path (lpath lidx)) = [lidx].
+proof.
+move=> rg_lidx @/leaves_from_path; rewrite size_lpath_lt 1:/# /=.
+have h_gt0 := h_g0; rewrite iftrue 1:/# mkseq1 /=.
+by rewrite /lpath revK BS2Int.int2bsK /#.
+qed.
+
+lemma lfp_nil : leaves_from_path [] = range 0 (2^h).
+proof.
+have h_gt0 := h_g0; rewrite /leaves_from_path ifT 1:/# /=.
+by rewrite rev_nil BS2Int.bs2int_nil /= /mkseq id_map //#.
+qed.
+
+lemma lfp_st _lstart _sth:
+   leaves_from_path (prefix (lpath _lstart) _sth) = range _lstart (_lstart + 2 ^ _sth).
+admitted.
+
+(* The leaf node corresponding to a leaf path
+   The semantics of this needs to be computed from wots using
+   operators and then proved equivalent to the imperative code. *)
+op wots_pk_val(ss ps : Params.nbytes, ad : SA.adrs, lidx : int) : dgstblocklenlist =
+   pkWOTS_from_skWOTS (gen_skWOTS ss ps ad) ps ad.
+
+op leafnode_from_idx(ss ps : Params.nbytes, ad : adrs, lidx : int) : dgstblock =
+ let pk = wots_pk_val ss ps (set_kpidx (set_typeidx ad 0) lidx) lidx in
+ bs2block (ltree ps (ads2adr (set_kpidx (set_typeidx ad 1) lidx))
+           (LenNBytes.insubd (map NBytes.insubd (chunk n (BitsToBytes (flatten (map DigestBlock.val (DBLL.val pk)))))))).
+(*
+lemma Eqv_Ltree_ltree (pkWOTS : wots_pk) (ad : adrs) (ps : seed) :
+  phoare[LTree.ltree : arg = (pkWOTS, ad, ps) ==> ltree ps ad pkWOTS = res] = 1%r.
+conseq (: _ ==> true) (: _ ==> _);1,2:smt(); last first.
++ proc.
+  wp; while (true) (_len).
+  + move => *.
+    wp;while (true) (_len %/ 2 - i).
+    move => *.
+    inline *;auto => /> /#.
+  by auto => /> /#.
+ by auto => /> /#.
+proc *. ecall (ltree_eq _seed address pk).
+by auto => />.
+qed.
+*)
+
+lemma Eqv_WOTS_pkgen  (ad : adrs) (ss ps : seed) :
+  hoare[WOTS.pkGen : arg = (ss, ps, ads2adr ad) ==>
+     LenNBytes.insubd (map NBytes.insubd (chunk n (BitsToBytes (flatten (map DigestBlock.val (DBLL.val
+       (pkWOTS_from_skWOTS (gen_skWOTS ss ps ad) ps ad))))))) = res].
+admitted.
+
+lemma Eqv_WOTS_pkgen_ll  :
+ islossless WOTS.pkGen.
+admitted.
+
+(* list of all the leaves up to an index, exclusive *)
+op leaf_range(ss ps : Params.nbytes, ad : SA.adrs, start lidxo  : int) =
+   map (leafnode_from_idx ss ps ad) (range start lidxo).
+
+lemma leaf_range0 ss ps ad s : 0 <= s => leaf_range ss ps ad s 0 = [].
+proof. move => *; by rewrite /leaf_range range_geq. qed.
+
+(* The node corresponding to an arbitrary path  *)
+op node_from_path (p : bool list, ss ps : Params.nbytes, ad : SA.adrs) : dgstblock =
+ if size p = h
+ then leafnode_from_idx ss ps ad (BS2Int.bs2int (rev p))
+ else if 0 <= size p <= h
+      then let ls = leaves_from_path p in
+           let nls = map (leafnode_from_idx ss ps ad) ls in
+           let subtree = list2tree nls in
+               (val_bt_trh subtree ps (set_typeidx ad trhtype)
+                   (h - size p) (head witness ls))
+      else witness.
+
+(* The full stack state when one starts to process leaf lidx *)
+op stack_from_leaf (start lidxo t : int, ss ps : Params.nbytes, ad : SA.adrs) : (dgstblock * int) list =
+  map (fun p => (node_from_path (prefix (lpath start) t ++ p) ss ps ad,  t - size p)) (paths_from_leaf lidxo t).
+
+lemma sfl_size start lidxo t ss ps ad :
+    0 <= t <= h
+ => 0 <= start <= 2^h - 2^t
+ => 2^t %| start
+ => 0 <= lidxo <= 2^t
+ => size (stack_from_leaf start lidxo t ss ps ad) = hw (lpathst lidxo t).
+proof. move=> *; rewrite /stack_from_leaf size_map pfl_size //. qed.
+
+(* The list of leaves that fall under the first node in the stack when one starts to process leaf lidx
+   The case o lidx=0 is a corner case, as the stack is empty *)
+op first_subtree_leaves(start lidxo t : int,ss ps : Params.nbytes, ad : SA.adrs) =
+ if lidxo = 0 then
+   []
+ else
+   let lps = (paths_from_leaf lidxo t) in
+   let p1 = prefix (lpath start) t ++ head witness lps in
+   let lp1 = leaves_from_path p1 in
+   map (leafnode_from_idx ss ps ad) lp1.
+
+(* The hamming weight of 0 is 0, so stack is empty *)
+lemma pfl0 t :
+    0 <= t <= h
+ =>   paths_from_leaf 0 t = [].
+proof.
+move => *;have expr_gt0 := expr_gt0; apply/size_eq0.
+rewrite pfl_size //= 1:/#.
+by rewrite /lpathst /= BS2Int.int2bs0 /= /hw count_rev count_nseq /pred1 //=.
+qed.
+
+lemma stack_from_leaf0 start t ss ps ad :
+    0 <= t <= h
+ => 0 <= start <= 2^h - 2^t
+ => 2^t %| start
+ => stack_from_leaf start 0 t ss ps ad = [].
+proof. move => *;rewrite /stack_from_leaf pfl0 //. qed.
+
+(* This op describes the state of the stack in the inner loop, while
+   reducing, where o is the current offset = size of stack = sfl ++ [rednode].
+   There are two cases: either the hw increased by one, then there
+   is nothing to do. Or it has decreased and we enter the loop.
+   The loop performs as many iterations as needed to reduce the
+   hamming weight of lidx to hamming weight of lidx+1, if any. *)
+op stack_increment (start lidxo t : int, ss ps : Params.nbytes, ad : SA.adrs, offset : int) =
+  (* the stack configuration is the state encountered for lidx
+     with the extra node computed for lidx at the end *)
+  let hwi = hw (lpathst lidxo t) in
+  let hwi1 = hw (lpathst (lidxo + 1) t) in
+  if hwi < hwi1
+  (* Then then case only happens when lidx is even, in which
+     case we are already in the state we need on exit *)
+  then stack_from_leaf start lidxo t ss ps ad ++
+          [(node_from_path (lpath (start +lidxo)) ss ps ad, 0)]
+  else
+      (* we reach this point with hw1 <= offset <= hw + 1
+         we still did not touch the first (offset - 1) positions in the old stack
+         the node stored at offset - 1 corresponds to the node reduced along the
+         path to lidx that we can also compute *)
+      let oldstack = stack_from_leaf start lidxo t ss ps ad in
+      let level = if offset = size oldstack + 1
+                  then 0 (* we always start reducing with a leaf *)
+                  else (nth witness oldstack (offset - 1)).`2 + 1 in
+      let carrypath = (take (h - level) (lpath (start + lidxo)))
+      in (take (offset - 1) oldstack) ++
+                        [(node_from_path carrypath ss ps ad, level)].
+
+
+lemma int2bs_enlarge (N1 N2 k : int) :
+  0 <= N1 <= N2 => 0 <= k < 2^N1 =>
+    BS2Int.int2bs N2 k = BS2Int.int2bs N1 k ++ nseq (N2 - N1) false.
+proof.
+move=> [ge0_N1 leN] [ge0_k ltk]; apply/(eq_from_nth false).
+- by rewrite size_cat size_nseq !BS2Int.size_int2bs 1:/#.
+rewrite BS2Int.size_int2bs lez_maxr 1:/# => i rgi.
+rewrite nth_cat BS2Int.size_int2bs lez_maxr //.
+case: (i < N1) => [lt_iN1|ge_iN1].
+- by rewrite /int2bs !nth_mkseq /= //#.
+rewrite /int2bs nth_mkseq ?nth_nseq /= ~-1://#.
+rewrite pdiv_small // ge0_k /=; suff: 2^N1 <= 2^i by smt().
+by apply: ler_weexpn2l => //#.
+qed.
+
+lemma hw_cat_pow2 (N k n1 n2 : int) :
+     0 <= N
+  => 0 <= k
+  => 0 <= n1
+  => 0 <= n2 < 2^k
+  => (n1 * 2^k + n2) < 2^N
+  =>   hw (BS2Int.int2bs N (n1 * 2^k + n2))
+     = hw (BS2Int.int2bs N n1) + hw (BS2Int.int2bs N n2).
+proof.
+have ? := expr_gt0; move=> *.
+case: (n1 = 0) => [->/=|nz_n1]; first by rewrite BS2Int.int2bs0 hw_nseq.
+have ?: k < N.
+- apply/ltrNge/negP => le_Nk.
+  have ?: 2^N <= 2^k by apply: ler_weexpn2l.
+  smt().
+rewrite (BS2Int.int2bs_cat k N) ~-1:/# hw_cat addrC; congr.
+- rewrite divzMDl 1:/# pdiv_small //=.
+  rewrite (int2bs_enlarge (N - k) N) 1://#.
+  - split=> // _; apply: (ltr_pmul2r (2^k)); first smt().
+    by rewrite -exprD_nneg //#.
+  by rewrite hw_cat hw_nseq /= /#.
+- rewrite -BS2Int.int2bs_mod modzMDl pmod_small //.
+  by rewrite (int2bs_enlarge k N) ~-1://# hw_cat hw_nseq /= //#.
+qed.
+
+lemma int2bs_pow2B1 (N k : int) :
+  0 <= k <= N => BS2Int.int2bs N (2^k - 1) = nseq k true ++ nseq (N - k) false.
+proof.
+have ? := expr_gt0; move=> ?; apply: BS2Int.inj_bs2int_eqsize.
+- by rewrite BS2Int.size_int2bs size_cat !size_nseq /#.
+rewrite BS2Int.int2bsK 1:/#.
+- by split=> [|_]; [|rewrite ltzE /= &(ler_weexpn2l)]; smt().
+by apply/eq_sym/BS2Int.bs2int_cat_nseq_true_false.
+qed.
+
+lemma hw_pow2B1 (N k : int) :
+  0 <= k <= N => hw (BS2Int.int2bs N (2^k - 1)) = k.
+proof.
+move=> rg_k; rewrite int2bs_pow2B1 // /hw count_cat.
+by rewrite !count_nseq /pred1 /=; smt().
+qed.
+
+lemma int2bs_incSE (N lidx : int) :
+     0 <= N
+  => 0 <= lidx
+  => lidx + 1 < 2^N
+  => let k = argmax (fun i => take i (BS2Int.int2bs N lidx)) (all idfun) in
+        (   k < N
+         /\ (forall i, 0 <= i < k => nth false (BS2Int.int2bs N lidx) i)
+         /\ nth false (BS2Int.int2bs N lidx) k = false
+         /\ BS2Int.int2bs N lidx
+            = nseq k true ++ false :: drop (k + 1) (BS2Int.int2bs N lidx)
+         /\ BS2Int.int2bs N (lidx + 1)
+            = nseq k false ++ true :: drop (k + 1) (BS2Int.int2bs N lidx)).
+proof.
+have ? := expr_gt0; move=> ge0_N ge0_ldx lt_lidxS k.
+have lt_lidx: lidx < 2 ^ N by smt().
+have lt_lidx' : lidx < 2 ^ (N+1) by rewrite exprSr //#.
+move: @k; (pose f i := take i (BS2Int.int2bs N lidx)) => k.
+have: exists i, 0 <= i < N /\ nth false (BS2Int.int2bs N lidx) i = false.
+- suff: !all idfun (BS2Int.int2bs N lidx).
+  - rewrite -has_predC => /hasP[b] @/predC @/idfun /= [+ hNb].
+    move/nthP => /(_ false) []; rewrite BS2Int.size_int2bs.
+    by rewrite lez_maxr // => i0 [rg_i0 hi0]; exists i0 => /#.
+  apply/negP => hones; have: BS2Int.int2bs N lidx = nseq N true.
+  - apply/(eq_from_nth false); 1: by rewrite ?size_nseq BS2Int.size_int2bs.
+    rewrite BS2Int.size_int2bs lez_maxr // => i rgi.
+    rewrite nth_nseq //; move/List.allP: hones.
+    move/(_ (nth false (BS2Int.int2bs N lidx) i)).
+    move=> @/idfun /= -> //; apply/mem_nth.
+    by rewrite BS2Int.size_int2bs lez_maxr.
+  move/(congr1 BS2Int.bs2int); rewrite BS2Int.int2bsK ~-1://.
+  by rewrite BS2Int.bs2int_nseq_true //#.
+case=> i0 [rg_i0 hbit0].
+have := argmaxP_r f (List.all idfun) 0 N // _ _ _; 1,2: smt(take0).
+- move=> k0 rg_k0; rewrite -has_predC &(hasP).
+  exists (nth false (BS2Int.int2bs N lidx) i0).
+  rewrite -{1}(nth_take _ k0) ~-1:/# mem_nth /=.
+  - by rewrite size_take_condle ~-1:/# BS2Int.size_int2bs /#.
+  - by rewrite /predC /idfun /= hbit0.
+rewrite -/k => [# ge0_k allones hz]; have: k < N.
+- rewrite ltzNge; apply/negP => le_Nk.
+  move/all_nthP: allones => /(_ false i0 _).
+  - by rewrite size_take // BS2Int.size_int2bs /#.
+  by rewrite /idfun nth_take ~-1://# hbit0.
+move=> ^lt_kN -> /=; rewrite -!andaE.
+split=> [//|allones_k]; last split=> [|?].
+- move=> i [ge0_i lt_ik]; move/all_nthP: allones => /(_ false i _).
+  - by rewrite size_take_condle // BS2Int.size_int2bs /#.
+  by rewrite /idfun /= /f nth_take.
+- have := hz (k + 1) _; ~-1: smt().
+  rewrite -has_predC => /hasP[b] @/predC @/idfun.
+  case=> + hNb - @/f; rewrite (take_nth false).
+  - by rewrite ?BS2Int.size_int2bs //#.
+  rewrite mem_rcons /=; case=> [<-//#|hmemb].
+  by move/List.allP: allones => /(_ _ hmemb) /#.
+have: BS2Int.int2bs N lidx =
+  nseq k true ++ false :: BS2Int.int2bs (N - (k+1)) (lidx %/ 2^(k+1)).
+- apply/(eq_from_nth false).
+  - rewrite size_cat /= !BS2Int.size_int2bs /= size_nseq /#.
+  rewrite BS2Int.size_int2bs lez_maxr // => i rgi.
+  rewrite nth_cat size_nseq lez_maxr //; case: (i < k).
+  - by move=> lt_ik; rewrite nth_nseq ~-1:/# allones_k //#.
+  move=> /lerNgt le_ki; case: (i = k) => /= [->>//|].
+  move=> ne_ik; rewrite subr_eq0 ne_ik /=.
+  rewrite (BS2Int.int2bs_cat (k+1) N) ~-1:/#.
+  rewrite nth_cat BS2Int.size_int2bs lez_maxr ~-1://#.
+  by rewrite iffalse 1:/# opprD !addrA.
+move=> ^eq {1}->; split.
+- do 2! congr; rewrite !drop_mkseq 1:/# &(eq_in_mkseq) /(\o) /=.
+  by move=> i rgi; rewrite -divz_mul 1:/# -exprD_nneg ~-1://#.
+move=> _; move/(congr1 BS2Int.bs2int): eq; rewrite BS2Int.int2bsK ~-1://#.
+rewrite -cat1s catA BS2Int.bs2int_cat -nseq1.
+rewrite {1}(_ : 1 = (k + 1) - k) 1:#ring.
+rewrite BS2Int.bs2int_cat_nseq_true_false ~-1:/#.
+rewrite size_cat !size_nseq /= !lez_maxr ~-1:/#.
+rewrite BS2Int.int2bsK 1:/#; first split=> [|_].
+- by rewrite divz_ge0 // expr_gt0.
+- rewrite ltz_divLR; first smt(expr_gt0).
+  by rewrite -exprD_nneg //#.
+move/(congr1 (fun i => i + 1))=> /= ->.
+rewrite (BS2Int.int2bs_cat (k+1) N) ~-1:/#.
+rewrite addrAC /= -BS2Int.int2bs_mod.
+rewrite {1}[2^(k+1)*_]mulrC modzMDr.
+rewrite pmod_small 1:exprSr ~-1://#.
+rewrite BS2Int.int2bs_pow2 ?mem_range ~-1://# /=.
+rewrite nseq0 -catA cat1s /=; do 2? congr.
+rewrite [2^(k+1)*_]mulrC divzMDr ~-1:/#.
+rewrite [2^_ %/ _]pdiv_small 1:exprSr ~-1://# /=.
+apply/(eq_from_nth false).
+- by rewrite size_drop ~-1://# !BS2Int.size_int2bs /#.
+rewrite ?BS2Int.size_int2bs lez_maxr 1:/# => i rgi.
+rewrite nth_drop ~-1:/# /int2bs !nth_mkseq ~-1://# /=.
+rewrite -divzMr; ~-1:smt(expr_gt0).
+by rewrite -exprD_nneg //#.
+qed.
+
+lemma hwincSE (N lidx : int) :
+     0 <= N
+  => 0 <= lidx
+  => lidx + 1 < 2^N
+  => let k = argmax (fun i => take i (BS2Int.int2bs N lidx)) (all idfun) in
+     hw (BS2Int.int2bs N (lidx + 1)) = hw (BS2Int.int2bs N lidx) + 1 - k.
+proof.
+have ? := h_g0; move=> 3? k; have := int2bs_incSE N lidx _ _ _ => //.
+have ge0_k: 0 <= k by apply: ge0_argmax.
+rewrite -/k /= => -[# lekN hones hzero _ ->]; rewrite hw_cat /= hw_nseq //=.
+rewrite -{2}[BS2Int.int2bs N _](cat_take_drop (k+1)).
+rewrite hw_cat /= [hw (take _ _)](_ : _ = k) -1:#ring.
+rewrite [take _ _](_ : _ = rcons (nseq k true) false); last first.
+- by rewrite -cats1 hw_cat hw_nseq //=; smt(ge0_argmax).
+rewrite (take_nth false) ?BS2Int.size_int2bs ~-1://#; congr.
+have sztk: size (take k (BS2Int.int2bs N lidx)) = k.
+- by rewrite size_take_condle // BS2Int.size_int2bs /#.
+rewrite &(eq_from_nth false) ?size_nseq 1:/# sztk.
+move=> i [ge0_i ltik]; rewrite nth_nseq //.
+by rewrite nth_take // hones.
+qed.
+
+lemma hwincSE_lpathst (lidxo t : int) :
+    0 <= t <= h
+ => 0 <= lidxo < 2^t =>
+     (   lidxo = 2^t - 1
+      /\ lpathst lidxo t = nseq t true
+      /\ lpathst (lidxo + 1) t = true :: nseq t false)
+  \/ (   lidxo < 2^t - 1
+      /\ let k = argmax (fun i => take i (BS2Int.int2bs t lidxo)) (all idfun) in
+         hw (lpathst (lidxo + 1) t) = hw (lpathst lidxo t) + 1 - k).
+proof.
+move => ?;case=> rg0_lidx /ltzE /lez_eqVlt [SlidxE | lt_Slidx]; [left | right].
+- have ->/=: lidxo = 2^t - 1 by apply/Ring.IntID.subr_eq.
+  rewrite /lpathst !int2bs_pow2B1 /=; ~-1:smt(h_g0).
+  rewrite b2i0_eq 1:/# /= nseq0 cats0 rev_nseq /=.
+  rewrite BS2Int.int2bs_pow2 /=;1:smt(mem_range).
+  by rewrite nseq0 /= rev_cat rev_nseq rev1 //.
+- split=> [/# | k @/lpath]; rewrite !hw_rev.
+  rewrite [lidxo + 1 = _]ltr_eqF // [lidxo = _]ltr_eqF 1:/#.
+  by have /= := hwincSE t lidxo _ _ _;smt().
+qed.
+
+(* hw increases by exactly 1 *)
+lemma hwinc lidxo t :
+    0 <= t <= h
+ => 0 <= lidxo < 2^t
+   => hw (lpathst lidxo t) < hw (lpathst (lidxo+1) t)
+   => hw (lpathst (lidxo+1) t) = hw (lpathst lidxo t) + 1.
+proof.
+move=> ?;case => *. 
+have := hwincSE_lpathst lidxo t _ _;1,2:smt().
+smt(ge0_argmax hw_nseq).
+qed.
+
+(* we don't enter the loop if hw increased *)
+lemma hwinc_noentry start lidxo t ss ps ad offset:
+    0 <= t <= h
+ => 0 <= start <= 2^h - 2^t
+ => 2^t %| start
+ => 0 <= lidxo < 2^t =>
+    hw (lpathst lidxo t) < hw (lpathst (lidxo + 1) t) =>
+   let si = stack_increment start lidxo t ss ps ad offset in
+    ((size si < 2) \/
+     (2 <= size si /\
+       (nth witness si (size si - 1)).`2 <>
+         (nth witness si (size si - 2)).`2)).
+move=> tr sr tdiv lt hinc si; have siE: si =
+  stack_from_leaf start lidxo t ss ps ad ++ [(node_from_path (lpath (start+lidxo)) ss ps ad, 0)].
+- by rewrite /si /stack_increment /=; rewrite hinc.
+have ? := h_g0; move: lt hinc => ^[ge0_lidx _]; case/(hwincSE_lpathst lidxo t tr).
+- move=> [# + -> ->] /= -; rewrite !hw_nseq /= 1,2: /#.
+  move => ??;rewrite /si; have -> : lidxo = 0 by smt(Ring.IntID.expr0).
+  left; rewrite /stack_increment /= /lpathst /= /stack_from_leaf /=/paths_from_leaf /= /extract_path /=.
+  have -> /= : b2i (0 = 2 ^ t) = 0 by smt(Ring.IntID.expr0).
+  have -> /= : b2i (1 = 2 ^ t) = 1 by smt(Ring.IntID.expr0).
+  rewrite !BS2Int.int2bs0 /= !BS2Int.int2bs1 /= 1:/#.
+  have ->  /=: hw (rev (nseq t false)) < hw (rev (true :: nseq t false)). 
+  + by rewrite /hw rev_cons !rev_nseq -cats1 count_cat /= !count_nseq /#.
+  have -> /= : (0 = 2 ^ t) = false by smt(Ring.IntID.expr0).
+  rewrite size_cat size_map pmap_map size_map /= /lpathst /= size_filter count_map /preim /=.
+  have -> /= : b2i (0 = 2 ^ t) = 0 by smt(Ring.IntID.expr0).
+  rewrite count_pred0_eq_in; last by smt().
+  move => *; rewrite !BS2Int.int2bs0 /= /extract_path rev_nseq /predC1 /= ifF; last by smt(). 
+  smt(nth_nseq_if).
+(pose k':= argmax _ _) => [# /= *].
+have := int2bs_incSE t lidxo _ _ _; ~-1: by move=> //#.
+rewrite -/k' /= => [#] _ _ /=.
+have ->: k' = 0 by smt(ge0_argmax).
+rewrite nseq0 /= nth0_head => hhd eqE.
+case: (size si < 2) => /= [//|/lezNgt ^ge2_sz -> /=].
+rewrite nth_last {1}siE last_cat /= eq_sym.
+have ?: 0 < size (stack_from_leaf start lidxo t ss ps ad).
+- by move: ge2_sz; rewrite siE size_cat /= /#.
+pose d := (nth witness si (size si - 2)).`2.
+have: d \in map snd (stack_from_leaf start lidxo t ss ps ad).
+- apply/(@map_f snd); rewrite siE nth_cat size_cat /= iftrue 1:/#.
+  apply/mem_nth; smt().
+rewrite /stack_from_leaf -map_comp /(\o) /= => /mapP /=.
+case=> p [+ ->] - @/paths_from_leaf; case: (lidxo = _) => /= [->/=|].
++ smt(Ring.IntID.expr0).
+case/pmapP=> i [/mem_range rgi] @/extract_path.
+case: (nth false (lpathst lidxo t) i) => // nthi /someI ->.
+rewrite size_rcons size_take ~-1:/# size_lpathst ~-1:/#.
+rewrite [lidxo = _]ltr_eqF 1:/# /= iftrue 1:/#.
+suff: i <> t - 1 by smt().
+apply: contraL nthi => ->; rewrite {2}(_ : t = size (lpathst lidxo t)).
+- by rewrite size_lpathst /#. 
+by rewrite nth_last /lpath last_rev b2i0_eq 1:/# /= hhd.
+qed.
+
+(* hw increase implies odd, so last node in paths is the previous leaf *)
+lemma hwinc_leaflast lidxo t : 
+    0 <= t <= h 
+ => 0 <= lidxo < 2^t 
+   => hw (lpathst lidxo t) < hw (lpathst (lidxo + 1) t)
+   =>    size (nth witness (paths_from_leaf (lidxo + 1) t) (hw (lpathst lidxo t))) = t
+      /\ lidxo = BS2Int.bs2int (rev (nth witness (paths_from_leaf (lidxo + 1) t) (hw (lpathst (lidxo + 1) t) - 1))).
+proof.
+move=> tr lt hinc.
+case (t = 0).
++ move => Ht;rewrite Ht /=;have Hlidxo : lidxo = 0 by smt(Ring.IntID.expr0).
+  by rewrite /paths_from_leaf !Hlidxo /= /lpathst /= BS2Int.int2bs0 BS2Int.int2bs1 1:/# /= nseq0 /=  rev1  /= rev_nil BS2Int.bs2int_nil /=.
+move => tg0.
+ move: lt hinc => ^[ge0_lidx _]; case/(hwincSE_lpathst lidxo t tr).
+- move=> [# + -> ->] /= - -> /=; rewrite !hw_nseq /= // 1,2:/# => tl1.
+  rewrite ifT 1:/# /= rev_nil BS2Int.bs2int_nil;smt(Ring.IntID.expr0). 
+(pose k':= argmax _ _) => [# /= *].
+have := int2bs_incSE t lidxo _ _ _; ~-1: by move=> //#.
+rewrite -/k' /= => [#] _ _ /=.
+have ->: k' = 0 by smt(ge0_argmax).
+move=> + _ +; rewrite nseq0 /= nth0_head => hhd eqE.
+rewrite /paths_from_leaf !iffalse ~-1:/#.
+pose p1 := lpathst (lidxo + 1) t; pose p2 := lpathst lidxo t.
+have: exists s, size s = t - 1 /\ ((p1 = rcons s true) /\ (p2 = rcons s false)). (* FACTOR OUT *)
+- exists (rev (drop 1 (BS2Int.int2bs t lidxo))); split.
+  - by rewrite size_rev size_drop // BS2Int.size_int2bs;smt(Ring.IntID.expr0). 
+  split.
+  - by rewrite /p1 /lpathst ltr_eqF 1:/# /= eqE rev_cons.
+  - rewrite /p2 /lpathst ltr_eqF 1:/# /= -rev_cons; congr.
+    rewrite -{1}[BS2Int.int2bs _ _](cat_take_drop 1) -cat1s; congr.
+    rewrite -[BS2Int.int2bs _ _]drop0 (drop_take1_nth false) /=.
+    - by rewrite BS2Int.size_int2bs /#.
+    - by rewrite nth0_head.
+case=> s [szs [^p1E-> ^p2E->]]; rewrite !hw_rcons /=.
+have ->: nth witness (pmap (extract_path (rcons s true)) (range 0 t)) (hw s) = rcons s false.
+- rewrite (range_cat (t - 1)) ~-1:/# pmap_cat nth_cat.
+  rewrite pfl_r_size_min ~-1:/# (_ : take (t - 1) (rcons s true) = s).
+  - by rewrite -cats1 take_cat szs /= cats0.
+  rewrite ltrr /= (rangeS (t - 1)) /= /extract_path.
+  rewrite nth_rcons szs /= -[rcons s true]cats1 take_cat.
+  by rewrite szs /= cats0.
+rewrite size_rcons szs /= rev_rcons.
+move/(congr1 rev)/(congr1 BS2Int.bs2int): p2E.
+rewrite /p2 rev_rcons => <- @/lpath; rewrite revK.
+by rewrite [lidxo = 2^t]ltr_eqF 1:/# /= BS2Int.int2bsK //#.
+qed.
+
+
+(* hw increase implies all previous paths same as before *)
+lemma hwinc_pathsprev lidxo t k :
+    0 <= t <= h
+ => 0 <= lidxo < 2^t =>
+    hw (lpathst lidxo t) < hw (lpathst (lidxo  + 1) t) =>
+     0 <= k < hw (lpathst lidxo t) =>
+      (nth witness (paths_from_leaf (lidxo  + 1) t) k)
+      = (nth witness (paths_from_leaf lidxo t) k).
+proof.
+move=> tr lt hinc.
+case (t = 0).
++ move => Ht;rewrite Ht /=;have Hlidxo : lidxo = 0 by smt(Ring.IntID.expr0).
+  rewrite /paths_from_leaf !Hlidxo /= /lpathst /= BS2Int.int2bs0 nseq0 /=.
+  rewrite rev_nil /hw /= /#. 
+move => tg0.
+ move: lt hinc => ^[ge0_lidx _]; case/(hwincSE_lpathst lidxo t tr).
+- move=> [# + -> ->] /= - -> /=; rewrite !hw_nseq /= // /#.
+(pose k':= argmax _ _) => [# /= *].
+have := int2bs_incSE t lidxo _ _ _; ~-1: by move=> //#.
+rewrite -/k' /= => [#] _ _ /=.
+have ->: k' = 0 by smt(ge0_argmax).
+move=> + _ +; rewrite nseq0 /= nth0_head => hhd eqE.
+rewrite /paths_from_leaf !iffalse ~-1://#.
+pose p1 := lpathst (lidxo + 1) t; pose p2 := lpathst lidxo t.
+have: exists s, size s = t - 1 /\ ((p1 = rcons s true) /\ (p2 = rcons s false)).
+- exists (rev (drop 1 (BS2Int.int2bs t lidxo))); split.
+  - by rewrite size_rev size_drop // BS2Int.size_int2bs /#.
+  split.
+  - by rewrite /p1 /lpathst ltr_eqF 1:/# /= eqE rev_cons.
+  - rewrite /p2 /lpathst ltr_eqF 1:/# /= -rev_cons; congr.
+    rewrite -{1}[BS2Int.int2bs _ _](cat_take_drop 1) -cat1s; congr.
+    rewrite -[BS2Int.int2bs _ _]drop0 (drop_take1_nth false) /=.
+    - by rewrite BS2Int.size_int2bs /#.
+    - by rewrite nth0_head.
+case=> s [szs [^p1E-> ^p2E->]].
+pose s1 := pmap (extract_path _) _.
+pose s2 := pmap (extract_path _) _.
+suff: take (k+1) s1 = take (k+1) s2.
+- move/(congr1 (fun s => nth witness s k)) => /=.
+  by rewrite !nth_take ~-1://#.
+have lek: k < hw s.
+- have: k < hw (lpathst lidxo t) by smt().
+  by rewrite -/p2 p2E hw_rcons /=.
+apply: pfl_eq; first 2 smt().
+- move=> n ge0_n; rewrite -!cats1 !take_cat.
+  by case: (n < size s) => /=; rewrite ?hw_cat; smt().
+- by rewrite hw_rcons /= /#.
+- by rewrite hw_rcons /= /#.
+qed.
+
+(* hw decrease implies odd, so last node in old stack is leaf *)
+lemma hwnoinc_leaflast lidxo t :
+    0 <= t <= h
+ => 0 <= lidxo < 2^t =>
+    hw (lpathst (lidxo  + 1) t) <= hw (lpathst lidxo t)  =>
+     (0 < hw (lpathst lidxo t) /\
+     size (nth witness (paths_from_leaf lidxo t) ((size (paths_from_leaf lidxo t)) - 1)) = t).
+proof.
+move=> tr lt hinc.
+have Ht : 0 < t. 
++  case (t  = 0) => /= H; 2: smt().
+   move : hinc; have -> /= : lidxo = 0 by smt(Ring.IntID.expr0).
+   rewrite H /lpathst /hw /= BS2Int.int2bs0 /= !nseq0 rev_nil /=.
+   by rewrite BS2Int.int2bs1 //= nseq0 /= rev1 /= /#.
+ move: lt hinc => ^[ge0_lidx _]; case/(hwincSE_lpathst lidxo t tr).
+- move=> [# + -> ->] /= - -> /=; rewrite !hw_nseq /= //= 1,2:/# => lt1.
+  split;1:smt(). 
+  rewrite /paths_from_leaf /= ifF 1:/# /= nth_last /extract_path pmap_map /=. 
+  rewrite -last_map -map_comp.
+  have [#[H1 _]]:= all_filterP (predC1 None) (map
+           (fun (i : int) =>
+              if nth false (lpathst (2 ^ t - 1) t) i then Some (rcons (take i (lpathst (2 ^ t - 1) t)) false) else None)
+           (range 0 t)).
+  rewrite H1.
+  + rewrite /predC1 all_map /preim /= allP => x ? /=; rewrite ifT;last by smt().
+    rewrite /lpathst /=.
+    have-> /=: b2i (2 ^ t - 1 = 2 ^ t) = 0 by smt().
+    rewrite BS2Int.int2bs_cat_nseq_true_false 1:/# /= nseq0 cats0 /= rev_nseq.
+    by rewrite nth_nseq_if;smt(mem_range). 
+  rewrite -map_comp /(\o) /=.
+  rewrite (range_cat (t-1) 0 t) 1,2:/# map_cat.
+  have -> : (range (t-1) t)  = (range (t-1) ((t-1) + 1)) by smt().
+  rewrite rangeS /= -cat_rcons cats0 last_rcons.
+  rewrite ifT.
+  + rewrite /lpathst.
+    have-> /=: b2i (2 ^ t - 1 = 2 ^ t) = 0 by smt().
+    rewrite BS2Int.int2bs_cat_nseq_true_false 1:/# /= nseq0 cats0 /= rev_nseq.
+    by rewrite nth_nseq_if;smt(mem_range). 
+  rewrite oget_some /= size_rcons /= size_take 1:/#.
+  rewrite /lpathst.
+  have-> /=: b2i (2 ^ t - 1 = 2 ^ t) = 0 by smt().
+  rewrite BS2Int.int2bs_cat_nseq_true_false 1:/# /= nseq0 cats0 /= rev_nseq.
+  by rewrite size_nseq /#.
+(pose k':= argmax _ _) => [# /= ? -> ?]; have ?: 0 < k' by smt().
+have := int2bs_incSE t lidxo _ _ _; ~-1: by move=> //#.
+rewrite -/k' /= => [#] _ _ /= => hhd eqE1 eqE2; split.
+- rewrite /lpath hw_rev b2i0_eq 1:/# /=.
+  by rewrite eqE1 hw_cat /= hw_nseq ~-1:/# /=; smt(ge0_hw).
+rewrite pfl_size 1:/# /paths_from_leaf 1:/# iffalse 1:/#.
+rewrite /lpathst hw_rev b2i0_eq 1:/# /=.
+rewrite -hw_rev; have <- := pfl_r_size (rev (BS2Int.int2bs t lidxo)) t.
+- by rewrite size_rev BS2Int.size_int2bs //#.
+rewrite nth_last (range_cat (t - 1)) ~-1:/# pmap_cat rangeS /=.
+pose q := extract_path _ (t - 1).
+suff ->/=: q = Some (rcons (take (t - 1) (rev (BS2Int.int2bs t lidxo))) false).
+- rewrite last_cat /= size_rcons size_take_condle ~-1:/#.
+  by rewrite size_rev BS2Int.size_int2bs /#.
+rewrite /q /extract_path /= nth_rev ?BS2Int.size_int2bs 1:/# /=.
+rewrite lez_maxr 1:/# /= iftrue // eqE1 nth_cat.
+by rewrite size_nseq iftrue ~-1:/# nth_nseq /#.
+qed.
+
+lemma take_nseq ['a] (i j : int) (x : 'a) : 0 <= i <= j =>
+  take i (nseq j x) = nseq i x.
+proof. by move=> rg; rewrite -!mkseq_nseq take_mkseq. qed.
+
+(* if inner loop exited, then we have reached the final stack size *)
+lemma hwdec_exit start lidxo t ss ps ad offset :
+    0 <= t <= h
+ => 0 <= start <= 2^h - 2^t
+ => 2^t %| start
+ => 0 <= lidxo < 2^t
+   => hw (lpathst (lidxo + 1) t) <= hw (lpathst lidxo t)
+   => hw (lpathst (lidxo + 1) t) <= offset <= hw (lpathst lidxo t) + 1
+   => let si = stack_increment start lidxo t ss ps ad offset in
+      (   size si < 2
+       \/ (2 <= size si /\ (nth witness si (size si - 1)).`2 <> (nth witness si (size si - 2)).`2))
+   => offset = hw (lpathst (lidxo + 1) t) /\ size si = hw (lpathst (lidxo + 1) t).
+proof.
+move=> tr sr ds lt hinc.
+case (t = 0). admit.
+move => gt0t.
+ move: lt hinc => ^[ge0_lidx _]; case/(hwincSE_lpathst lidxo t tr).
+- admit.
+(pose k':= argmax _ _) => [# /=] ? + ^hdec - -> ?.
+have ?: 0 < k' by smt().
+have := int2bs_incSE t lidxo _ _ _; ~-1: by move=> //#.
+rewrite -/k' /= => [#] ?? /= => hhd eqE1 eqE2 hoff.
+pose si := stack_increment _ _ _ _ _ _ _.
+print stack_increment.
+pose oldstack := stack_from_leaf start lidxo t ss ps ad.
+pose level :=
+  if   offset = size oldstack + 1
+  then 0
+  else (nth witness oldstack (offset - 1)).`2 + 1.
+pose carrypath := take (h - level) (lpath (start + lidxo)).
+have siE : si =
+  take (offset - 1) oldstack ++ [(node_from_path carrypath ss ps ad, level)].
+- by rewrite /si /stack_increment /= iffalse //= /#.
+move=> hsz; rewrite -andaE; split; last first.
+- rewrite siE => -> /=; rewrite size_cat /= size_take_condle.
+  - rewrite /lpathst hw_rev b2i0_eq 1:/# /=.
+    by rewrite eqE1 hw_cat /= hw_nseq 1:/# /=; smt(ge0_hw).
+  by rewrite sfl_size 1..4:/# iftrue /#.
+have szod: size oldstack = hw (lpathst lidxo t). 
+- by rewrite /oldstack sfl_size /#.
+have ltk': k' <= hw (lpathst lidxo t).
+- rewrite /lpathst hw_rev b2i0_eq 1:/# /= eqE1.
+  by rewrite hw_cat hw_nseq 1:/# /=; smt(ge0_hw).
+have nthod: forall i, 0 <= i < k' => (nth witness (rev oldstack) i).`2 = i.
+- move=> i rgi; rewrite nth_rev /oldstack sfl_size ~-1:/#.
+  rewrite /stack_from_leaf (nth_map witness) 1:pfl_size ~-1:/# /=.
+  rewrite /paths_from_leaf iffalse 1:/# (range_cat (t - (i+1))) ~-1:/#.
+  have eqsz: hw (lpathst lidxo t) - (i + 1) =
+    size (pmap (extract_path (lpathst lidxo t)) (range 0 (t - (i + 1)))).
+  - rewrite &(eq_sym) /= pfl_r_size_min 1:/# {2}/lpathst b2i0_eq 1:/# /=.
+    rewrite -[BS2Int.int2bs _ _](cat_take_drop (i + 1)).
+    rewrite rev_cat 2?(rev_take, rev_drop) ?BS2Int.size_int2bs ~-1:/#.
+    rewrite lez_maxr 1:/# hw_cat /lpathst b2i0_eq 1:/# /=.
+    rewrite -addrA -{1}[hw _]addr0; congr; apply/eq_sym.
+    rewrite {1}[t](_ : _ = size (BS2Int.int2bs t lidxo)).
+    - by rewrite BS2Int.size_int2bs /#.
+    rewrite -rev_take ?BS2Int.size_int2bs 1:/# hw_rev eqE1.
+    rewrite take_cat' take_nseq ~-1:/# hw_cat hw_nseq /= 1:/#.
+    by rewrite size_nseq iftrue 1:/# /=.
+  rewrite pmap_cat nth_cat iffalse; first by rewrite eqsz.
+  rewrite eqsz /= range_ltn 1:/# /=.
+  have ->/=: extract_path (lpathst lidxo t) (t - (i + 1)) =
+    Some (rcons (take (t - (i + 1)) (lpathst lidxo t)) false).
+  - rewrite /extract_path iftrue //= /lpathst nth_rev.
+    - by rewrite BS2Int.size_int2bs /= b2i0_eq /#.
+    rewrite b2i0_eq 1:/# BS2Int.size_int2bs lez_maxr 1:/# /=.
+    rewrite [t - _](_ : _ = i) 1:#ring eqE1 nth_cat.
+    by rewrite size_nseq iftrue 1:/# nth_nseq //#.
+  by rewrite size_rcons /= size_take 1:/# size_lpathst /#.
+case: hoff; rewrite ler_eqVlt; case=> // gtoff leoff; suff //: false.
+have ge2_offset: 2 <= offset by smt().
+have size_tk_od: size (take (offset - 1) oldstack) = offset - 1.
+- by rewrite /oldstack size_take_condle -1:sfl_size -1:iftrue //#.
+have ge2_szsi: 2 <= size si by rewrite siE size_cat /= size_tk_od.
+move: hsz; rewrite ltrNge ge2_szsi /= nth_last {1}siE last_cat /=.
+rewrite {1}siE cats1 nth_rcons iftrue; first by rewrite siE size_cat /#.
+rewrite siE size_cat /= nth_take ~-1:/# size_tk_od /=.
+have := nthod (size oldstack - (offset - 1)) _; first smt().
+rewrite nth_rev /= 1:/# !(opprB, opprD, addrA) /= => ->.
+rewrite /level; case: (offset = size oldstack + 1) => [->//|neoff].
+have := nthod (size oldstack - offset) _; first smt().
+by rewrite nth_rev /= 1:/# !opprD !addrA /= => ->; ring.
+qed.
+
+(* final state of stack after reduction *)
+lemma stack_final start lidxo t ss ps ad :
+    0 <= t <= h
+ => 0 <= start <= 2^h - 2^t
+ => 2^t %| start
+ => 0 <= lidxo < 2^t =>
+   forall k, 0 <= k < hw (lpathst (lidxo  + 1) t) =>
+         nth witness (stack_increment start lidxo t ss ps ad (hw (lpathst (lidxo + 1) t)))  k
+       = nth witness (stack_from_leaf start (lidxo + 1) t ss ps ad) k.
+proof.
+move => ???? k *.
+case (hw (lpathst (lidxo + 1) t) <= hw (lpathst lidxo t)) => *;last first.
++ rewrite /stack_increment /= ifT 1:/#.
+  rewrite nth_cat sfl_size 1..4:/#.
+  case (k < hw (lpathst lidxo t)) => *.
+  +  have := hwinc_pathsprev  lidxo t k _ _ _. smt(). smt(). smt().
+     rewrite /stack_from_leaf !(nth_map witness) /=; smt(pfl_size).
+  rewrite ifT;1:smt(hwinc).
+  have ->: k = hw (lpathst (lidxo + 1) t) - 1 by smt(hwinc).
+  rewrite /stack_from_leaf !(nth_map witness) /=;1: smt(pfl_size).
+  have := hwinc_leaflast lidxo t _ _ _;1..3: smt().
+  move => [H H1];split; last  by smt(hwinc pfl_size).
+  admit.
+admitted.
+
+lemma si_size_in_loop start lidxo t ss ps ad offset :
+    0 <= t <= h
+ => 0 <= start <= 2^h - 2^t
+ => 2^t %| start
+ => 0 <= lidxo < 2^t =>
+hw (lpathst (lidxo + 1) t) <= hw (lpathst lidxo t) =>
+hw (lpathst (lidxo + 1) t) <= offset <= hw (lpathst lidxo t) + 1 =>
+2 <= offset =>
+(nth witness (stack_increment start lidxo t ss ps ad offset) (offset - 1)).`2 = 
+(nth witness (stack_increment start lidxo t ss ps ad offset) (offset - 2)).`2 =>
+   size ((stack_increment start lidxo t ss ps ad offset)) = offset /\
+   size (stack_from_leaf start (lidxo + 1) t ss ps ad) < offset.
+admitted.
+(*
+move => *;split.
++ move => *; rewrite /stack_increment /= ifF 1:/#.
+  rewrite size_cat /= size_take 1:/#.
+  smt(sfl_size).
+admit. (* not finished yet *)
+qed. *)
+
+
+(* entering the inner loop for a leaf tree means that
+   we are still hashing values at height < h-1: when
+   we exit the loop for leaf 2^h - 1 we have produced a
+   hash at level h *)
+lemma si_heights_in_loop_bnd start lidxo t ss ps ad offset k :
+    0 <= t <= h
+ => 0 <= start <= 2^h - 2^t
+ => 2^t %| start
+ => 0 <= lidxo < 2^t =>
+hw (lpathst (lidxo + 1) t) <= hw (lpathst lidxo t) =>
+2 <= offset =>
+(nth witness (stack_increment start lidxo t ss ps ad offset) (offset - 1)).`2 = 
+(nth witness (stack_increment start lidxo t ss ps ad offset) (offset - 2)).`2 =>
+0<= k < offset =>
+ 0<= (nth witness
+   (stack_increment start lidxo t ss ps ad offset) k).`2 < h.
+proof.
+move => *.
+admitted.
+
+(* In the inner loop, the final node in the stack
+  is the hash of the last two nodes in the previous
+  stack
+lemma si_reduced_node start lidxo t ss ps ad offset :
+  0 <= t <= h
+  => 0 <= start <= 2^h - 2^t
+  => 2^t %| start
+  => 0 <= lidxo < 2^t =>
+  hw (lpathst start (lidxo + 1) t) <= hw (lpathst start lidxo t) =>
+  2 <= offset =>
+  (nth witness (stack_increment start lidxo t ss ps ad offset) (offset - 1)).`2 =
+  (nth witness (stack_increment start lidxo t ss ps ad offset) (offset - 2)).`2 =>
+  let si = (stack_increment start lidxo t ss ps ad offset) in
+  let si1 = (stack_increment start lidxo t ss ps ad (offset - 1)) in
+  (nth witness si1 (offset - 2)).`1 =
+  trh ps (set_tree_index (set_tree_height (set_type zero_address 2) ((nth witness si (offset - 1)).`2))
+          ((start + lidxo) %/ 2 ^ ((nth witness si (offset - 1)).`2 + 1)))
+          ( (DigestBlock.val (nth witness si (offset - 2)).`1) ++
+           (DigestBlock.val (nth witness si (offset - 1)).`1)).
+proof.
+move => ? Hw ?? /=.
+admitted.
+*)
+lemma si_reduced_node start lidxo t ss ps ad offset :
+  0 <= t <= h
+  => 0 <= start <= 2^h - 2^t
+  => 2^t %| start
+  => 0 <= lidxo < 2^t =>
+  hw (lpathst (lidxo + 1) t) <= hw (lpathst lidxo t) =>
+  2 <= offset =>
+  (nth witness (stack_increment start lidxo t ss ps ad offset) (offset - 1)).`2 =
+  (nth witness (stack_increment start lidxo t ss ps ad offset) (offset - 2)).`2 =>
+  let si = (stack_increment start lidxo t ss ps ad offset) in
+  let si1 = (stack_increment start lidxo t ss ps ad (offset - 1)) in
+  (nth witness si1 (offset - 2)).`1 =
+  trh ps (set_thtbidx (set_typeidx (adr2ads zero_address) trhtype)
+          (nth witness si (offset - 1)).`2 ((start + lidxo) %/ 2 ^ ((nth witness si (offset - 1)).`2 + 1)))
+          ( (DigestBlock.val (nth witness si (offset - 2)).`1) ++
+           (DigestBlock.val (nth witness si (offset - 1)).`1)).
+proof.
+move => ? Hw ?? /=.
+admitted.
+
+(* growth of leaves under the leftmost subtree *)
+lemma growth ss ps ad leaves start lidxo t :
+    0 <= t <= h
+ => 0 <= start <= 2^h - 2^t
+ => 2^t %| start
+ => 0 <= lidxo < 2^t =>
+size leaves = lidxo =>
+ take (size (first_subtree_leaves start (size leaves) t ss ps ad)) leaves =
+   first_subtree_leaves start (size leaves) t ss ps ad =>
+ take (size (first_subtree_leaves start (lidxo + 1) t ss ps ad))
+   (rcons leaves (leafnode_from_idx ss ps ad (start + lidxo))) =
+ first_subtree_leaves start (lidxo + 1) t ss ps ad.
+admitted.
+
+(*
+phoare leaves_correct _ps _ss  _ad :
+ [ FL_XMSS_TW_ES.leaves_from_sspsad :
+  arg = (_ss, _ps, _ad)  ==>
+   res =
+  map
+    (leafnode_from_idx (NBytes.insubd (NBytes.val _ss)) (NBytes.insubd (NBytes.val _ps))
+       (set_layer_addr zero_address 0)) (range 0 (2 ^ h)) ] = 1%r.
+admitted.
+*)
+
+phoare leaves_correct _ps _ss  _ad :
+ [ FL_XMSS_TW_ES.leaves_from_sspsad :
+  arg = (_ss, _ps, _ad)  ==>
+   res =
+  map
+    (leafnode_from_idx (NBytes.insubd (NBytes.val _ss)) (NBytes.insubd (NBytes.val _ps)) _ad)
+      (range 0 (2 ^ h)) ] = 1%r.
+admitted.
+
+(*
+phoare tree_hash_correct _ps _ss _lstart _sth _ad :
+[ XMSS_TreeHash.TreeHash.treehash :
+    arg = (_ps,_ss,_lstart,_sth,_ad)
+/\  _ad = zero_address /\ 0 <= _sth <= h /\ 0 <= _lstart <= 2^h - 2^_sth  /\ 2^_sth %| _lstart 
+ ==>
+  DigestBlock.insubd (BytesToBits (NBytes.val res)) =  
+    val_bt_trh (list2tree (map (leafnode_from_idx _ss _ps _ad) 
+     (range  _lstart (_lstart + 2^_sth)))) _ps (set_typeidx zero_address trhtype) _sth _lstart  ] = 1%r.
+proof.
+conseq (: _ ==> true) (: _ ==> _);1,2:smt(); last first. 
++ proc. 
+  wp;while (true) (2^t - i).
+  + move => *; wp; while (true) (to_uint offset).
+    + move => *;inline *; auto => &hr;rewrite uleE /= => *. 
+      rewrite W64.to_uintB => /=;1: by rewrite uleE /= /#.
+      by smt().
+    wp;call(:true).
+    wp; while (true) (_len).
+    + move => *.
+      wp;while (true) (_len %/ 2 - i).
+      move => *.
+      inline *;auto => /> /#.
+    by auto => /> /#.
+   by auto => /> /#. 
+  sp;wp;exlim sk_seed, pub_seed, address => ss ps ad. 
+  call Eqv_WOTS_pkgen_ll.
+  + auto => /> &hr ? h o; rewrite uleE /=;split; smt(W64.to_uint_cmp).
+  by auto => /> /#.
+
+proc => /=.    
+wp;while ( #{/~_ad = zero_address}{~address = _ad}pre
+    /\ 0 <= i <= 2^t 
+    /\ (forall k, 0<=k<3 => address.[k] = W32.zero)
+    /\  size stack = h + 1 /\ size heights = h + 1
+    /\ (let stacklist = stack_from_leaf _lstart i _sth _ss _ps _ad in
+      to_uint offset = size stacklist /\
+      forall k, 0 <= k < size stacklist =>
+        bs2block (nth witness stack k) =
+          (nth witness stacklist k).`1 /\
+        to_uint (nth witness heights k) =
+          (nth witness stacklist k).`2)); last first.
++ auto => /> &1 *; do split.
+  + by smt(expr_ge0).
+  + by smt(Array8.initiE Array8.get_setE).
+  + by smt(size_nseq).
+  + by smt(size_nseq).
+  + by rewrite stack_from_leaf0 /#. 
+  + by move=> 2?; rewrite stack_from_leaf0 /= /#.
+  + move => ad hs i o st 7? H.
+    have @/bs2block -> := (H 0 _) => /=.
+    have -> : i = 2^_sth by smt(). 
+    rewrite sfl_size 1..4:/#; have-> := lpathst_root _lstart _sth _ _ _;1..3:smt(). 
+    rewrite /hw /=;smt(count_ge0).
+  + rewrite /stack_from_leaf nth0_head /paths_from_leaf /= ifT 1:/# /= cats0 /=.
+    rewrite /node_from_path. 
+    case (_sth = h) => Ht.
+    +  rewrite /prefix ifF;1:by smt(size_lpath StdOrder.IntOrder.expr_gt0 h_g0 take0).  
+       rewrite ifT /=;1:by smt(size_lpath StdOrder.IntOrder.expr_gt0 h_g0 take0).    
+       congr; -2: by smt(take_size size_take size_ge0 size_lpath StdOrder.IntOrder.expr_gt0). 
+       congr;congr; smt(lfp_st).
+       rewrite lfp_st /range iotaS_minus;smt(StdOrder.IntOrder.expr_gt0).
+    case (_sth = 0) => H0. 
+    +  rewrite /prefix ifT;1:smt(take_size size_take size_ge0 size_lpath StdOrder.IntOrder.expr_gt0 h_g0). 
+       have -> /= : (range _lstart (_lstart + 2 ^ _sth)) = [_lstart] by rewrite H0 /= rangeS.
+        rewrite H0 list2tree1 /=;congr.
+        rewrite take_size /lpath revK BS2Int.int2bsK;smt(h_g0 StdOrder.IntOrder.expr_gt0).
+    rewrite /prefix ifF;1:by smt(take_size size_take size_ge0 size_lpath StdOrder.IntOrder.expr_gt0 h_g0).  
+    rewrite ifT /=;1:by smt(take_size size_take size_ge0 size_lpath StdOrder.IntOrder.expr_gt0 h_g0). 
+    congr; -2: by smt(take_size size_take size_ge0 size_lpath StdOrder.IntOrder.expr_gt0). 
+    congr;congr; smt(lfp_st).
+    by rewrite lfp_st /range iotaS_minus;smt(StdOrder.IntOrder.expr_gt0).
+
+seq 6 : (#pre /\
+   bs2block node = leafnode_from_idx _ss _ps _ad (_lstart + i)).  
++ seq 3 : (#pre /\   pk = LenNBytes.insubd
+  (map NBytes.insubd
+     (chunk n
+        (BitsToBytes
+           (flatten (map DigestBlock.val (DBLL.val (wots_pk_val _ss _ps (set_kpidx (set_typeidx _ad 0) (_lstart + i)) (_lstart + i))))))))).
+  + conseq />;1: smt().
+    ecall (Eqv_WOTS_pkgen address sk_seed  pub_seed ).
+    auto => /> &1 &2 ????????????;split;1:smt(Array8.get_setE). 
+    congr;congr;congr;congr;congr;congr;congr. 
+    + rewrite /wots_pk_val;congr. 
+      + congr. admit. (* address semantics *)
+    rewrite /set_ots_addr /set_kpidx /set_idx.  admit. (* address semantics *)
+  ecall  (ltree_eq  pub_seed address  pk ).
+  auto => /> &1 &2 ????????????;split;1: by move => *; rewrite /set_ltree_addr /set_type; smt(Array8.get_setE).
+  rewrite /leafnode_from_idx /= /bs2block;congr;congr;congr;congr. 
+  +  rewrite /set_ltree_addr /set_kpidx /set_idx. admit.  (* address semantics *)
+
+wp. 
+while (
+ pub_seed = _ps /\
+     sk_seed = _ss /\
+     s = _lstart /\
+     t = _sth /\ 0 <= _sth /\ _sth <= h /\ 0 <= _lstart /\ _lstart <= 2 ^ h - 2 ^ _sth /\ 2 ^ _sth %| _lstart /\ 
+    0 <= i <= 2 ^ t 
+ /\   (hw (lpathst _lstart i _sth) < hw (lpathst _lstart (i + 1) _sth) => to_uint offset = hw (lpathst _lstart (i + 1) _sth)) 
+ /\ (hw (lpathst _lstart (i + 1) _sth) <= hw (lpathst _lstart i _sth) => 
+         hw (lpathst _lstart (i + 1) _sth) <= to_uint offset <= hw (lpathst _lstart i _sth) + 1)
+ /\size stack = h + 1 /\ size heights = h + 1 
+ /\ (forall k, (0<=k<5 \/ k=7) => address.[k] = (set_type zero_address 2).[k])
+ /\   0 <= i < 2 ^ t /\ t = _sth /\ s = _lstart 
+ /\ (let stacklist = 
+      stack_increment _lstart i _sth _ss _ps _ad (to_uint offset) in
+        to_uint offset = size stacklist
+      /\ forall (k : int), 0 <= k < size stacklist =>
+          bs2block (nth witness stack k) = (nth witness stacklist k).`1 /\
+          to_uint (nth witness heights k) = (nth witness stacklist k).`2)); last first.
++ auto => /> &2 ??????????Ho Hs?Hn. 
+  have -> /= : offset{2} + W64.one - W64.one = offset{2} by ring.
+  rewrite /= !W64.to_uintD_small /=. 
+  +  rewrite Ho sfl_size;   smt(size_lpathst count_size BS2Int.size_int2bs h_max).
+split. 
+(* initialization of inner loop invariant *)
++ rewrite /stack_increment /=.
+  pose _olds := (stack_from_leaf _lstart i{2} _sth _ss _ps _ad).
+  pose _hw1 := (hw (lpathst _lstart (i{2} + 1) _sth)).
+  pose _hw := (hw (lpathst _lstart i{2} _sth)).
+  have Hsos : size _olds = _hw
+      by rewrite /olds /stack_from_leaf size_map; smt(pfl_size h_g0).
+  do split.
++ smt(hwinc sfl_size). 
++ by smt(sfl_size).
++ by smt(size_put).
++ by smt(size_put).
++ move => k kb; rewrite /set_type /zero_address. 
+  by rewrite !get_setE 1..10:/#; smt(Array8.initiE).
++ case (_hw < _hw1).
+  + by rewrite size_cat;smt(hwinc).
+  by move => ?;rewrite  size_cat /= size_take; smt(W64.to_uint_cmp). 
++ move => k kbl kbh.
+  case (_hw < _hw1) => /= Hw.
+  + (* hw increased by 1, so we have to show that the previous stack plus
+         the new leaf is really the stack that we will end up with *)
+      rewrite !nth_put;1,2:by rewrite Ho sfl_size; smt(size_lpathst size_ge0 size_rev count_size BS2Int.size_int2bs).
+      rewrite nth_cat. 
+      case(to_uint offset{2} = k) => Hk.
+      + (* this is the leaf just added *)
+        rewrite ifF 1:/# ifT 1:/# /= Hn /node_from_path /= ifT;1:smt(size_lpath).
+        rewrite revK BS2Int.int2bsK /#.
+      + (* this is the previous stack *)
+        rewrite ifT;1:smt(sfl_size size_cat). 
+        move : (Hs k _);1:  smt(sfl_size size_cat).  
+        move => [-> ->]. 
+        by rewrite /stack_from_leaf !(nth_map witness) /=;smt(sfl_size pfl_size size_cat).
+    + (* reductions will be needed, but we haven't started
+         so we have the old stack in the first positions and a
+         new leaf at the next position *)
+      move : kbh; rewrite Hw /= !size_cat size_take;1:smt(W64.to_uint_cmp). 
+      rewrite ifF /=;1: smt(sfl_size).
+      move => kbh;rewrite !nth_cat /=. 
+      rewrite take_oversize;1:smt().
+      case (k < size _olds) => *; 1: by
+       rewrite !nth_put;smt(size_lpathst size_ge0 size_rev count_size BS2Int.size_int2bs sfl_size).
+      rewrite ifT;1: smt(sfl_size size_cat).
+      rewrite ifT;1: smt(sfl_size size_cat).
+      have -> /= : k = to_uint offset{2}  by smt(sfl_size).
+      rewrite !nth_put /=;1,2: by rewrite Ho sfl_size 1:/# /hw /lpath; smt(size_lpathst size_ge0 size_rev count_size BS2Int.size_int2bs).
+      rewrite take_oversize; 1: smt(size_lpath).
+      rewrite /node_from_path ifT;1: smt(size_lpath).
+      rewrite Hn;congr.
+      by rewrite /lpath revK /= BS2Int.int2bsK /#.
+
+move => ad hs o s.
++ rewrite uleE /= => Hout. 
+  have Hout' : to_uint o < 2 \/ (2 <= to_uint o /\ nth witness hs (to_uint o - 1) <> nth witness hs (to_uint o - 2)).
+  + case (to_uint o < 2) => /= *; 1: by smt(). 
+    move : Hout;rewrite !to_uintB /=;1,2: by rewrite uleE /= /#. 
+    by smt().
+ 
+  move => ???? Ha2 Ho2  H5.
+  rewrite /stack_increment /=.
+  pose _hw1 := (hw (lpathst _lstart (i{2} + 1) _sth)).
+  pose _hw := (hw (lpathst _lstart (i{2}) _sth)).
+do split.
+  + by smt(size_rcons).
+  + by smt().
+  + move => k kbl kbh; rewrite Ha2 1:/#.
+    rewrite /set_type /zero_address. 
+    by rewrite !get_setE 1..5:/#; smt(Array8.initiE).
+  + case (_hw < _hw1) => *;1: by smt(sfl_size).
+    have /= := hwdec_exit _lstart i{2} _sth _ss _ps _ad (to_uint o) _ _ _ _;1..4:smt().
+    + have ->  :size (stack_increment _lstart i{2} _sth _ss _ps _ad (to_uint o)) = to_uint o by smt().
+      move : Hout'. 
+      case (to_uint o < 2) => /=*;1:  smt(sfl_size size_lpathst size_ge0 size_rev count_size BS2Int.size_int2bs).
+   by smt(W32.to_uint_eq sfl_size W64.to_uint_cmp sfl_size hwinc).
+   
+  + case (_hw < _hw1) => ? k *.
+    + case (k < _hw) => *. 
+      + have ? := hwinc_pathsprev _lstart i{2} _sth k _ _ _ _ _ _;1..6: smt().
+        have ? := hwinc_leaflast  _lstart i{2} _sth _ _ _ _ _;1..5: smt(). 
+        by rewrite -!stack_final;smt().
+      by rewrite !H5;smt(W32.to_uint_eq sfl_size W64.to_uint_cmp stack_final).
+  + have /= := hwdec_exit  _lstart i{2} _sth _ss _ps _ad (to_uint o) _ _ _ _ _ _ _;1..6:smt(). 
+    + have ->  :size (stack_increment  _lstart i{2} _sth _ss _ps _ad (to_uint o)) = to_uint o by smt().
+      move : Hout'.
+      case (to_uint o < 2)  => /=*;1:smt().
+      by rewrite -!H5; smt(W32.to_uint_eq sfl_size W64.to_uint_cmp stack_final).
+     move => *.
+     rewrite !H5;1,2: smt(W32.to_uint_eq sfl_size W64.to_uint_cmp stack_final).
+      by smt(W32.to_uint_eq sfl_size W64.to_uint_cmp stack_final).
+
+seq 3  :
+  (#pre 
+  /\ address = set_tree_index 
+      (set_tree_height (set_type zero_address 2) (to_uint (nth witness heights (to_uint offset - 1)))) 
+        ((_lstart + i) %/ 2^(to_uint (nth witness heights (to_uint offset - 2)) + 1))).
++ auto => /> &hr ?????????????Ho Hs; rewrite uleE /= => H.
+  rewrite !to_uintB /=;1,2: by rewrite uleE /=; smt(). 
+  move => H1;rewrite H1.
+  move : (Hs (to_uint offset{hr} - 1) _);1: smt(sfl_size).
+  move : (Hs (to_uint offset{hr} - 2) _);1: smt(sfl_size).
+  move => [# Hs21 Hs22] [# Hs11 Hs12].
+
+have ? :  hw (lpathst _lstart (i{hr} + 1) _sth) <= hw (lpathst _lstart i{hr} _sth) by
+ have /=:= hwinc_noentry _lstart i{hr} _sth _ss _ps _ad (to_uint offset{hr}) _;smt(sfl_size). 
+
+have -> : 
+     (to_uint
+         (W32.of_int (_lstart + i{hr}) `>>`
+          truncateu8 ((nth witness heights{hr} (to_uint offset{hr} - 2) + W32.one) `&` W32.of_int 31))) = 
+     ((_lstart + i{hr})%/ 2^(to_uint (nth witness heights{hr} (to_uint offset{hr} - 2)) + 1)); last first.  
+  + split;1: by move => *;rewrite /set_tree_index /set_tree_height /=; smt(Array8.get_setE).
+    rewrite tP => k kb;rewrite /set_tree_index /set_tree_height /=.
+    pose x:= 
+       (stack_increment _lstart i{hr} _sth _ss _ps _ad (hw (lpathst _lstart i{hr} _sth) + 1 - to_uint offset{hr})).
+    pose y := W32.of_int ((_lstart + i{hr})  %/ 2^(to_uint (nth witness heights{hr} (to_uint offset{hr} - 2)) + 1)).
+     case (0<=k<5 \/ k= 7);1:by smt(Array8.get_setE).
+     case (k=6);1:by smt(Array8.get_setE).
+     move => *; have -> : k=5 by smt(). 
+     rewrite !get_setE //= /#. 
+
+  + rewrite /(`>>`) /= to_uint_truncateu8.
+    have -> : 31 = 2^5 - 1 by rewrite /=.
+    rewrite and_mod //= to_uintD_small /=   Hs22 /=.
+    + by have := si_heights_in_loop_bnd _lstart i{hr} _sth _ss _ps _ad (to_uint offset{hr})  (to_uint offset{hr} - 2) _ _ _;smt(h_max). 
+    rewrite to_uint_shr /=;1: smt(W32.to_uint_cmp).
+    rewrite of_uintK  modz_small => /=;1: smt(l_max).
+    rewrite of_uintK  modz_small /= 1:/#. 
+    rewrite modz_small 1:/#.
+    by rewrite modz_small;
+     have := si_heights_in_loop_bnd _lstart i{hr} _sth _ss _ps _ad (to_uint offset{hr})  (to_uint offset{hr} - 2) _ _ _;smt(h_max).
+  
+seq 3 : (#pre /\ 
+   node0 = nth XMSS_TreeHash.nbytes_witness stack (to_uint offset - 2)
+/\  node1 = nth XMSS_TreeHash.nbytes_witness stack (to_uint offset - 1)   
+/\   new_node = block2bs  (trh _ps (set_tree_index (set_tree_height (set_type zero_address 2) (to_uint (nth witness heights{hr} (to_uint offset{hr} - 1))))
+  ((_lstart + i{hr}) %/ 2 ^ (to_uint (nth witness heights{hr} (to_uint offset{hr} - 2)) + 1)) ) (BytesToBits (NBytes.val node0) ++ BytesToBits (NBytes.val node1)))).
++ inline *; auto => /> &hr ???????????????; rewrite uleE /= => ?. 
+   rewrite !to_uintB /=;1,2:by  rewrite ?uleE /=; smt().
+   move => ?.
+   rewrite /trh /thfc /= ifF. smt(@StdOrder gt0_n gt2_len).
+   rewrite /block2bs DigestBlock.insubdK. 
+   + rewrite /BytesToBits (size_flatten_ctt 8);1:smt(mapP W8.size_w2bits).
+     rewrite size_map;1: smt(NBytes.valP).
+   rewrite BytesToBitsK NBytes.valKd /rand_hash /=.
+   congr.
+
+     have Hs8 :  (size (BytesToBits (NBytes.val (nth XMSS_TreeHash.nbytes_witness stack{hr} (to_uint offset{hr} - 2)))) %/ 8) = size (chunk 8 (BytesToBits (NBytes.val (nth XMSS_TreeHash.nbytes_witness stack{hr} (to_uint offset{hr} - 2)))))     by rewrite size_chunk //.
+
+  have Hsd : (size (BytesToBits (NBytes.val (nth XMSS_TreeHash.nbytes_witness stack{hr} (to_uint offset{hr} - 2)))) +
+       size (BytesToBits (NBytes.val (nth XMSS_TreeHash.nbytes_witness stack{hr} (to_uint offset{hr} - 1))))) %/
+      8 %/ 2 = size (BytesToBits (NBytes.val (nth XMSS_TreeHash.nbytes_witness stack{hr} (to_uint offset{hr} - 2)))) %/ 8.
+        + have -> : size (BytesToBits (NBytes.val (nth XMSS_TreeHash.nbytes_witness stack{hr} (to_uint offset{hr} - 1)))) =
+            size (BytesToBits (NBytes.val (nth XMSS_TreeHash.nbytes_witness stack{hr} (to_uint offset{hr} - 2)))); last by smt().
+          rewrite /BytesToBits !(size_flatten_ctt 8);1,2: smt(mapP W8.size_w2bits). 
+          by rewrite !size_map !NBytes.valP.
+
+     have ? : size
+  (map W8.bits2w
+     (take
+        (size
+           (BytesToBits (NBytes.val (nth XMSS_TreeHash.nbytes_witness stack{hr} (to_uint offset{hr} - 2))) ++
+            BytesToBits (NBytes.val (nth XMSS_TreeHash.nbytes_witness stack{hr} (to_uint offset{hr} - 1)))) %/
+         8 %/ 2)
+        (chunk 8
+           (BytesToBits (NBytes.val (nth XMSS_TreeHash.nbytes_witness stack{hr} (to_uint offset{hr} - 2))) ++
+            BytesToBits (NBytes.val (nth XMSS_TreeHash.nbytes_witness stack{hr} (to_uint offset{hr} - 1))))))) =
+n.
+     + rewrite size_map size_cat 1:Hsd chunk_cat;1: by rewrite /BytesToBits !(size_flatten_ctt 8); smt(mapP W8.size_w2bits). 
+       rewrite Hs8  take_cat' /= take0 /= cats0 /= take_size size_chunk //. 
+       rewrite /BytesToBits !(size_flatten_ctt 8);1: smt(mapP W8.size_w2bits). 
+       by rewrite !size_map !NBytes.valP /= /#.
+
+     have ? : size
+  (map W8.bits2w
+     (drop
+        (size
+           (BytesToBits (NBytes.val (nth XMSS_TreeHash.nbytes_witness stack{hr} (to_uint offset{hr} - 2))) ++
+            BytesToBits (NBytes.val (nth XMSS_TreeHash.nbytes_witness stack{hr} (to_uint offset{hr} - 1)))) %/
+         8 %/ 2)
+        (chunk 8
+           (BytesToBits (NBytes.val (nth XMSS_TreeHash.nbytes_witness stack{hr} (to_uint offset{hr} - 2))) ++
+            BytesToBits (NBytes.val (nth XMSS_TreeHash.nbytes_witness stack{hr} (to_uint offset{hr} - 1))))))) =
+n.
+     + rewrite size_map size_cat 1:Hsd chunk_cat;1: by rewrite /BytesToBits !(size_flatten_ctt 8); smt(mapP W8.size_w2bits). 
+       rewrite Hs8  drop_cat /= drop0 /= /BytesToBits flattenK //;1:smt(mapP W8.size_w2bits). 
+       by rewrite !size_map !NBytes.valP /= /#.
+
+congr;congr;congr;1,4..:by rewrite /prf.
+
+   + rewrite /BitsToBytes size_map size_chunk // -map_take.
+     rewrite NBytes.insubdK 1:/# map_take size_cat Hsd.
+     rewrite chunk_cat;1:by rewrite /BytesToBits !(size_flatten_ctt 8); smt(mapP W8.size_w2bits). 
+     rewrite map_cat Hs8 -(size_map W8.bits2w) take_cat' /= take0 cats0 take_size.
+     have ->: map W8.bits2w
+  (chunk 8 (BytesToBits (NBytes.val (nth XMSS_TreeHash.nbytes_witness stack{hr} (to_uint offset{hr} - 2))))) =
+     BitsToBytes (BytesToBits (NBytes.val (nth XMSS_TreeHash.nbytes_witness stack{hr} (to_uint offset{hr} - 2)))) by smt().
+     by rewrite BytesToBitsK.
+
+   + rewrite /BitsToBytes size_map size_chunk // -map_drop.
+     rewrite NBytes.insubdK 1:/# map_drop size_cat Hsd.
+     rewrite chunk_cat;1:by rewrite /BytesToBits !(size_flatten_ctt 8); smt(mapP W8.size_w2bits). 
+     rewrite map_cat Hs8 -(size_map W8.bits2w) drop_cat /= drop0 /=. 
+     have ->: map W8.bits2w
+  (chunk 8 (BytesToBits (NBytes.val (nth XMSS_TreeHash.nbytes_witness stack{hr} (to_uint offset{hr} - 1))))) =
+     BitsToBytes (BytesToBits (NBytes.val (nth XMSS_TreeHash.nbytes_witness stack{hr} (to_uint offset{hr} - 1)))) by smt().
+     by rewrite BytesToBitsK.
+
++ auto => /> &hr ?????????????Ho Hs; rewrite uleE /= => H.
+  rewrite !to_uintB /=;1..2,4: by rewrite uleE /=; smt(). 
+  + by rewrite uleE /= to_uintB /=; rewrite ?uleE /=; smt().
+  
+  move => H1;rewrite H1.
+  move : (Hs (to_uint offset{hr} - 1) _);1: smt(sfl_size).
+  move : (Hs (to_uint offset{hr} - 2) _);1: smt(sfl_size).
+  move => [# Hs21 Hs22] [# Hs11 Hs12].
+
+have ? :  hw (lpathst _lstart (i{hr} + 1) _sth) <= hw (lpathst _lstart i{hr} _sth) by
+ have /=:= hwinc_noentry _lstart i{hr} _sth _ss _ps _ad (to_uint offset{hr}) _;smt(). 
+
+split;1: smt().
+
+have Hsil := si_size_in_loop _lstart i{hr} _sth _ss _ps _ad (to_uint offset{hr}) _ _ _ _ _ _ _ _; 1..8: smt(). 
+
+  do split.
+  + move => *;split;2:smt().
+    rewrite Ho.
+    rewrite Ho /stack_increment /= ifF 1:/# ifF 1:/# /= !size_cat /=.
+    rewrite size_take;1:smt(size_ge0).
+    by  smt(sfl_size size_take).
+  + by smt(size_put).
+  + by smt(size_put).
+  + rewrite Ho /stack_increment /= ifF 1:/# /= !size_cat /=.
+    rewrite size_take;1:smt(size_ge0).
+    have -> /= : !(hw (lpathst _lstart i{hr} _sth) < hw (lpathst _lstart (i{hr} + 1) _sth)) by smt().
+    by case (to_uint offset{hr} - 1 < size (stack_from_leaf _lstart i{hr} _sth _ss _ps _ad));rewrite size_cat /=; by  smt(sfl_size size_take).
+
+  + move => k kbl kbh. 
+    rewrite !nth_put;1,2: smt(size_lpathst count_size BS2Int.size_int2bs size_rev).
+    have kbh1 : k < to_uint offset{hr} -1.
+    + move : kbh;rewrite /stack_increment /= ifF 1:/# size_cat /=.
+      smt(size_take sfl_size).
+    case (to_uint offset{hr} - 2 = k) => Hk; last first. 
+    + rewrite !Hs;1,2:smt().
+      rewrite /stack_increment /= ifF 1:/#.
+      have -> /= : !(hw (lpathst _lstart i{hr} _sth) < hw (lpathst _lstart (i{hr} + 1) _sth)) by smt().
+      rewrite !nth_cat /= ifT;1:smt(size_take sfl_size size_ge0).
+      have -> /=: !(k - size (take (to_uint offset{hr} - 2) (stack_from_leaf _lstart i{hr} _sth _ss _ps _ad)) = 0) by smt(sfl_size size_take).
+      rewrite !ifT;1:smt(size_take sfl_size size_ge0).
+      by rewrite !nth_take;smt(size_take sfl_size size_ge0). 
+   split. 
+  + rewrite /bs2block /block2bs NBytes.insubdK;1: 
+      by rewrite /BitsToBytes size_map size_chunk 1:/# DigestBlock.valP /#.   
+    rewrite BitsToBytesK;1: by rewrite DigestBlock.valP /=; smt().
+    rewrite DigestBlock.valKd /=.
+    have /= := si_reduced_node _lstart i{hr} _sth _ss _ps _ad (to_uint offset{hr}) _ _ _ _ _ _ _;1..7:smt().
+    rewrite Hk => ->; congr; 1: smt(). 
+    congr.
+    + rewrite -Hk -Hs21 /bs2block DigestBlock.insubdK.
+      + rewrite /BytesToBits (size_flatten_ctt 8);  smt(mapP W8.size_w2bits size_map NBytes.valP).
+      congr; congr; rewrite (nth_change_dfl XMSS_TreeHash.nbytes_witness witness);  smt(size_lpathst count_size BS2Int.size_int2bs size_rev).
+     rewrite  -Hs11 /bs2block DigestBlock.insubdK.
+      + rewrite /BytesToBits (size_flatten_ctt 8);  smt(mapP W8.size_w2bits size_map NBytes.valP).
+      congr; congr; rewrite (nth_change_dfl XMSS_TreeHash.nbytes_witness witness);  smt(size_lpathst count_size BS2Int.size_int2bs size_rev).
+  rewrite to_uintD_small /=.
+  + rewrite Hs22. 
+    + have := si_heights_in_loop_bnd _lstart i{hr} _sth _ss _ps _ad (to_uint offset{hr}) (to_uint offset{hr} - 2) _ _ _ _ _ _ _ _;smt(h_max).
+  rewrite Hs22.  
+    rewrite /stack_increment /= ifF 1:/# nth_cat /=.
+      have -> /= : !(hw (lpathst _lstart i{hr} _sth) < hw (lpathst _lstart (i{hr} + 1) _sth)) by smt().
+      rewrite !nth_cat /= ifT;1:smt(size_take sfl_size size_ge0).
+    rewrite ifF;1:smt(size_take sfl_size size_ge0).
+    rewrite ifT;1:smt(size_take sfl_size size_ge0).
+    rewrite ifF;1:smt(size_take sfl_size size_ge0).
+   rewrite /node_from_path /=.    
+   smt(nth_take).
+qed.
+*)
+
+lemma zeroadsE:
+  adr2ads zero_address = HAX.Adrs.insubd [0; 0; 0; 0].
+proof.
+rewrite /zero_address /adr2ads /adr2idxs; congr.
+rewrite &(eq_from_nth witness) /=; 1: smt(size_rev size_map size_sub).
+move=> i ?; rewrite nth_rev 2:(nth_map witness) 3:nth_sub; 1..3:smt(size_rev size_map size_sub).
+by rewrite size_map size_sub 1:// initE /= ifT; smt(size_rev size_map size_sub to_uint0).
+qed.
+
+lemma zeroadiP:
+  valid_adrsidxs [0; 0; 0; 0].
+proof. by smt(val_w ge2_len expr_gt0). qed.
+
+phoare tree_hash_correct _ps _ss _lstart _sth :
+  [ TreeHash.treehash :
+      arg = (_ps,_ss,_lstart,_sth, zero_address)
+  /\ 0 <= _sth <= h /\ 0 <= _lstart <= 2^h - 2^_sth  /\ 2^_sth %| _lstart
+ ==>
+  DigestBlock.insubd (BytesToBits (NBytes.val res)) =
+    val_bt_trh (list2tree (map (leafnode_from_idx _ss _ps (adr2ads zero_address))
+     (range _lstart (_lstart + 2^_sth)))) _ps (set_typeidx (adr2ads zero_address) trhtype) _sth _lstart  ] = 1%r.
+proof.
+conseq (: _ ==> true) (: _ ==> _);1,2:smt(); last first.
++ proc.
+  wp;while (true) (2^t - i).
+  + move => *; wp; while (true) (to_uint offset).
+    + move => *;inline *; auto => &hr;rewrite uleE /= => *.
+      rewrite W64.to_uintB => /=;1: by rewrite uleE /= /#.
+      by smt().
+    (*
+    wp;call(:true).
+    wp; while (true) (Params.len - i).
+    + move => *.
+      wp;while (true) (Params.len %/ 2 - i).
+      move => *.
+      inline *;auto => /> /#.
+    by auto => /> /#.
+   by auto => /> /#.
+   *)
+  sp;wp;exlim sk_seed, pub_seed, address => ss ps ad.
+  call Eqv_WOTS_pkgen_ll.
+  + auto => /> &hr ? h o; rewrite uleE /=;split; smt(W64.to_uint_cmp).
+  by auto => /> /#.
+
+proc => /=.
+wp;while ( #{/~address = zero_address}pre
+    /\ 0 <= i <= 2^t
+    /\ (forall k, 0 <= k < 3 => address.[k] = W32.zero)
+    /\ address.[7] = W32.zero
+    /\ size stack = h + 1 /\ size heights = h + 1
+    /\ (let stacklist = stack_from_leaf _lstart i _sth _ss _ps (adr2ads zero_address) in
+      to_uint offset = size stacklist /\
+      forall k, 0 <= k < size stacklist =>
+        bs2block (nth witness stack k) =
+          (nth witness stacklist k).`1 /\
+        to_uint (nth witness heights k) =
+          (nth witness stacklist k).`2)); last first.
++ auto => /> &1 *; do split.
+  + by smt(expr_ge0).
+  + by smt(Array8.initiE Array8.get_setE).
+  + by smt(size_nseq).
+  + by smt(size_nseq).
+  + by rewrite stack_from_leaf0 /#.
+  + by move=> 2?; rewrite stack_from_leaf0 /= /#.
+  + move => ad hs i o st 8? H.
+    have steq:
+      forall (tp : int), valid_typeidx tp =>
+        set_typeidx (adr2ads ad) tp = set_typeidx (adr2ads zero_address) tp.
+    + move=> tp valtp @/set_typeidx.
+      by congr; rewrite &(eq_from_nth witness); smt(nth_put size_put HAX.Adrs.valP).
+    have @/bs2block -> := (H 0 _) => /=.
+    have -> : i = 2^_sth by smt().
+    rewrite sfl_size 1..4:/#; have-> := lpathst_root _sth _;1:smt().
+    rewrite /hw /=;smt(count_ge0).
+  + rewrite /stack_from_leaf nth0_head /paths_from_leaf /= ifT 1:/# /= cats0 /=.
+    rewrite /node_from_path.
+    case (_sth = h) => Ht.
+    +  rewrite /prefix ifF;1:by smt(size_lpath StdOrder.IntOrder.expr_gt0 h_g0 take0).
+       rewrite ifT /=;1: by smt(size_lpath StdOrder.IntOrder.expr_gt0 h_g0 take0).
+       congr; 2,-2: by smt(take_size size_take size_ge0 size_lpath StdOrder.IntOrder.expr_gt0).
+       congr;congr; smt(lfp_st).
+       rewrite lfp_st /range iotaS_minus;smt(StdOrder.IntOrder.expr_gt0).
+    case (_sth = 0) => H0.
+    +  rewrite /prefix ifT;1:smt(take_size size_take size_ge0 size_lpath StdOrder.IntOrder.expr_gt0 h_g0).
+       have -> /= : (range _lstart (_lstart + 2 ^ _sth)) = [_lstart] by rewrite H0 /= rangeS.
+        rewrite H0 list2tree1 /=.
+        suff /#: BS2Int.bs2int (rev (take (size (lpath _lstart)) (lpath _lstart))) = _lstart.
+        rewrite take_size /lpath revK BS2Int.int2bsK;smt(h_g0 StdOrder.IntOrder.expr_gt0).
+    rewrite /prefix ifF;1:by smt(take_size size_take size_ge0 size_lpath StdOrder.IntOrder.expr_gt0 h_g0).
+    rewrite ifT /=;1:by smt(take_size size_take size_ge0 size_lpath StdOrder.IntOrder.expr_gt0 h_g0).
+    congr; 2,-2: by smt(take_size size_take size_ge0 size_lpath StdOrder.IntOrder.expr_gt0).
+    congr;congr; smt(lfp_st).
+    by rewrite lfp_st /range iotaS_minus;smt(StdOrder.IntOrder.expr_gt0).
+
+seq 6 : (#pre /\
+   bs2block node = leafnode_from_idx _ss _ps (adr2ads zero_address) (_lstart + i)).
++ seq 3 : (#pre /\   pk = LenNBytes.insubd
+  (map NBytes.insubd
+     (chunk n
+        (BitsToBytes
+           (flatten (map DigestBlock.val (DBLL.val (wots_pk_val _ss _ps (set_kpidx (set_typeidx (adr2ads zero_address) 0) (_lstart + i)) (_lstart + i))))))))).
+  + conseq />;1: smt().
+    ecall (Eqv_WOTS_pkgen (adr2ads address) sk_seed pub_seed).
+    auto => /> &1 &2 ?????????????; split.
+    rewrite adr2adsK 3://.
+    + by move => ii valii; smt(get_setE).
+    rewrite /valid_adrsidxs; split; 1: smt(size_rev size_map size_sub).
+    rewrite /valid_xidxvalslp /valid_xidxvalslpch; left.
+    rewrite ?nth_rev ?(nth_map witness); 1..12: smt(size_map size_sub).
+    rewrite /= /set_ots_addr /set_type ?size_map ?nth_iota ?size_iota 1..4:// /=.
+    rewrite ?get_setE // (: max 0 4 = 4) 1:// /= to_uintK_small; smt(l_max val_w ge2_len).
+    move => ?; split => [k ? ?|]; 1: by rewrite /set_ots_addr /set_type ?get_setE // /#.
+    congr;congr;congr;congr;congr;congr;congr.
+    + rewrite /wots_pk_val.
+      suff /#:
+        adr2ads (set_ots_addr (set_type address{1} 0) (_lstart + i{1})) =
+        set_kpidx (set_typeidx (adr2ads zero_address) 0) (_lstart + i{1}).
+      + rewrite zeroadsE /set_typeidx /set_kpidx HAX.Adrs.insubdK 1:zeroadiP /set_idx.
+        rewrite /put /= ifT 2:HAX.Adrs.insubdK 2:zeroadiP /=; 1: smt(HAX.Adrs.valP).
+        rewrite /adr2ads /adr2idxs; congr; apply (eq_from_nth witness); 1: smt(size_put size_rev size_map size_sub).
+        move=> ii rngi.
+        rewrite nth_rev 2:(nth_map witness) 3:nth_sub 4:?nth_put //; 1..3: smt(size_put size_rev size_map size_sub).
+        rewrite size_map size_sub 1:// /set_ots_addr /set_type ?get_setE 1..6://.
+        rewrite (: 3 + (4 - (ii + 1)) = 6 - ii) 1:/#.
+        case (ii <> 2) => /= [| -> /=].
+        smt(get_setE W32.to_uint0 size_rev size_map size_sub).
+        by rewrite to_uintK_small; smt(l_max).
+  (* ecall (ltree_eq pub_seed address  pk ). *)
+  auto => /> &1 &2 ???????????H?; do split.
+  + move=> k gek ltk.
+    by rewrite /set_ltree_addr /set_type; do ? rewrite get_setE 1:// ifF 1:/# => /#.
+  rewrite /leafnode_from_idx.
+  suff /#:
+    ads2adr (set_kpidx (set_typeidx (adr2ads zero_address) 1) (_lstart + i{1}))
+    =
+    set_ltree_addr (set_type address{1} 1) (_lstart + i{1}).
+  + rewrite zeroadsE /set_typeidx /set_kpidx HAX.Adrs.insubdK 1:zeroadiP /set_idx.
+    rewrite /put /= ifT 2:HAX.Adrs.insubdK /=; 1,2: smt(HAX.Adrs.valP).
+    rewrite /ads2adr /idxs2adr HAX.Adrs.insubdK 1:/#.
+    rewrite tP => ii rngii; rewrite initE rngii /=.
+    rewrite /set_ltree_addr /set_type.
+    rewrite ?get_setE // /#.
+(*
+  move=> k ge0_k ltszk.
+  move: (H k _); 1: smt(sfl_size).
+  move => ^ + -> => ->; split; do 2! congr.
+  rewrite /stack_from_leaf.
+  rewrite /node_from_path.
+  congr. rewrite fun_ext => p.
+  suff /#:
+    leafnode_from_idx _ss _ps (adr2ads address{1}) (BS2Int.bs2int (rev (prefix (lpath _lstart) _sth ++ p)))
+    =
+    leafnode_from_idx _ss _ps (adr2ads (set_ltree_addr (set_type address{1} 1) (_lstart + i{1})))
+          (BS2Int.bs2int (rev (prefix (lpath _lstart) _sth ++ p)))
+    /\
+    (let ls = leaves_from_path (prefix (lpath _lstart) _sth ++ p) in
+     let nls = map (leafnode_from_idx _ss _ps (adr2ads address{1})) ls in
+     let subtree = list2tree nls in
+     val_bt_trh subtree _ps (set_typeidx (adr2ads address{1}) trhtype) (h - size (prefix (lpath _lstart) _sth ++ p)) (head witness ls))
+    =
+    (let ls = leaves_from_path (prefix (lpath _lstart) _sth ++ p) in
+     let nls = map (leafnode_from_idx _ss _ps (adr2ads (set_ltree_addr (set_type address{1} 1) (_lstart + i{1})))) ls
+     in
+     let subtree = list2tree nls in
+     val_bt_trh subtree _ps (set_typeidx (adr2ads (set_ltree_addr (set_type address{1} 1) (_lstart + i{1}))) trhtype)
+       (h - size (prefix (lpath _lstart) _sth ++ p)) (head witness ls)).
+  admit. (* true: operators simply reset addresses *)
+  rewrite /stack_from_leaf.
+  rewrite /node_from_path.
+  congr. rewrite fun_ext => p.
+  suff /#:
+    leafnode_from_idx _ss _ps (adr2ads address{1}) (BS2Int.bs2int (rev (prefix (lpath _lstart) _sth ++ p)))
+    =
+    leafnode_from_idx _ss _ps (adr2ads (set_ltree_addr (set_type address{1} 1) (_lstart + i{1})))
+          (BS2Int.bs2int (rev (prefix (lpath _lstart) _sth ++ p)))
+    /\
+    (let ls = leaves_from_path (prefix (lpath _lstart) _sth ++ p) in
+     let nls = map (leafnode_from_idx _ss _ps (adr2ads address{1})) ls in
+     let subtree = list2tree nls in
+     val_bt_trh subtree _ps (set_typeidx (adr2ads address{1}) trhtype) (h - size (prefix (lpath _lstart) _sth ++ p)) (head witness ls))
+    =
+    (let ls = leaves_from_path (prefix (lpath _lstart) _sth ++ p) in
+     let nls = map (leafnode_from_idx _ss _ps (adr2ads (set_ltree_addr (set_type address{1} 1) (_lstart + i{1})))) ls
+     in
+     let subtree = list2tree nls in
+     val_bt_trh subtree _ps (set_typeidx (adr2ads (set_ltree_addr (set_type address{1} 1) (_lstart + i{1}))) trhtype)
+       (h - size (prefix (lpath _lstart) _sth ++ p)) (head witness ls)).
+  admit. (* true: operators simply reset addresses *)
+  rewrite /leafnode_from_idx /= /bs2block;congr;congr;congr;congr.
+  +  admit.  (* address semantics *)
+*)
+wp.
+while (
+ pub_seed = _ps /\
+     sk_seed = _ss /\
+     s = _lstart /\
+     t = _sth /\ 0 <= _sth /\ _sth <= h /\ 0 <= _lstart /\ _lstart <= 2 ^ h - 2 ^ _sth /\ 2 ^ _sth %| _lstart /\
+    0 <= i <= 2 ^ t
+ /\   (hw (lpathst i _sth) < hw (lpathst (i + 1) _sth) => to_uint offset = hw (lpathst (i + 1) _sth))
+ /\ (hw (lpathst (i + 1) _sth) <= hw (lpathst i _sth) =>
+         hw (lpathst (i + 1) _sth) <= to_uint offset <= hw (lpathst i _sth) + 1)
+ /\size stack = h + 1 /\ size heights = h + 1
+ /\ (forall k, (0<=k<5 \/ k=7) => address.[k] = (set_type zero_address 2).[k])
+ /\   0 <= i < 2 ^ t /\ t = _sth /\ s = _lstart
+ /\ (let stacklist =
+      stack_increment _lstart i _sth _ss _ps (adr2ads zero_address) (to_uint offset) in
+        to_uint offset = size stacklist
+      /\ forall (k : int), 0 <= k < size stacklist =>
+          bs2block (nth witness stack k) = (nth witness stacklist k).`1 /\
+          to_uint (nth witness heights k) = (nth witness stacklist k).`2)); last first.
++ auto => /> &2 ???????????Ho Hs?Hn.
+  have -> /= : offset{2} + W64.one - W64.one = offset{2} by ring.
+  rewrite /= !W64.to_uintD_small /=.
+  +  rewrite Ho sfl_size;   smt(size_lpathst count_size BS2Int.size_int2bs h_max).
+split.
+(* initialization of inner loop invariant *)
++ rewrite /stack_increment /=.
+  pose _olds := (stack_from_leaf _lstart i{2} _sth _ss _ps (adr2ads zero_address)).
+  pose _hw1 := (hw (lpathst (i{2} + 1) _sth)).
+  pose _hw := (hw (lpathst i{2} _sth)).
+  have Hsos : size _olds = _hw
+      by rewrite /olds /stack_from_leaf size_map; smt(pfl_size h_g0).
+  do split.
++ smt(hwinc sfl_size).
++ by smt(sfl_size).
++ by smt(size_put).
++ by smt(size_put).
++ move => k kb; rewrite /set_type /zero_address.
+  by rewrite !get_setE 1..10:/#; smt(Array8.initiE).
++ case (_hw < _hw1).
+  + rewrite size_cat; smt(hwinc sfl_size).
+  by move => ?;rewrite  size_cat /= size_take; smt(W64.to_uint_cmp sfl_size).
++ move => k kbl kbh.
+  case (_hw < _hw1) => /= Hw.
+  + (* hw increased by 1, so we have to show that the previous stack plus
+         the new leaf is really the stack that we will end up with *)
+      rewrite !nth_put;1,2:by rewrite Ho sfl_size; smt(size_lpathst size_ge0 size_rev count_size BS2Int.size_int2bs).
+      rewrite nth_cat.
+      case(to_uint offset{2} = k) => Hk.
+      + (* this is the leaf just added *)
+        rewrite ifF 2:ifT /=; 1,2: smt(sfl_size).
+        rewrite Hn /node_from_path /= ifT;1:smt(size_lpath).
+        rewrite revK BS2Int.int2bsK 1,2:/# //.
+      + (* this is the previous stack *)
+        rewrite ifT;1:smt(sfl_size size_cat).
+        move : (Hs k _);1:  smt(sfl_size size_cat).
+        move => [-> ->].
+          by rewrite /stack_from_leaf !(nth_map witness) /=; 1,2:smt(sfl_size pfl_size size_cat).
+    + (* reductions will be needed, but we haven't started
+         so we have the old stack in the first positions and a
+         new leaf at the next position *)
+      move : kbh; rewrite Hw /= !size_cat size_take;1:smt(W64.to_uint_cmp). 
+      rewrite ifF /=;1: smt(sfl_size).
+      move => kbh;rewrite !nth_cat /=.
+      rewrite take_oversize /_olds Ho; 1: smt(sfl_size).
+      case (k < size _olds) => *.
+      + rewrite !nth_put; 1,2: smt(size_lpathst size_ge0 size_rev count_size BS2Int.size_int2bs sfl_size).
+      rewrite ifF. smt(sfl_size size_ge0).
+      rewrite ifT. smt(sfl_size size_ge0).
+      rewrite ifF. smt(sfl_size size_ge0).
+      smt().
+      rewrite ifF. smt(size_lpath sfl_size size_ge0).
+      rewrite ifT. smt(size_lpath sfl_size size_ge0).
+      rewrite ifT. smt(size_lpath sfl_size size_ge0).
+      rewrite !nth_put; 1,2: rewrite sfl_size 1:/# /hw /lpath //; 1,2: smt(size_lpathst size_ge0 size_rev count_size BS2Int.size_int2bs).
+      rewrite take_oversize; 1: smt(size_lpath).
+      rewrite /node_from_path ifT;1: smt(size_lpath sfl_size).
+      rewrite Hn.
+      rewrite ifT. smt(size_lpath sfl_size size_ge0).
+      rewrite ifT. smt(size_lpath sfl_size size_ge0).
+      by rewrite /lpath revK /= BS2Int.int2bsK 1,2:/#.
+
+move => ad hs o s.
++ rewrite uleE /= => Hout.
+  have Hout' : to_uint o < 2 \/ (2 <= to_uint o /\ nth witness hs (to_uint o - 1) <> nth witness hs (to_uint o - 2)).
+  + case (to_uint o < 2) => /= *; 1: by smt().
+    move : Hout;rewrite !to_uintB /=;1,2: by rewrite uleE /= /#.
+    by smt().
+
+  move => ???? Ha2 Ho2  H5.
+  rewrite /stack_increment /=.
+  pose _hw1 := (hw (lpathst (i{2} + 1) _sth)).
+  pose _hw := (hw (lpathst (i{2}) _sth)).
+do split.
+  + by smt(size_rcons).
+  + by smt().
+  + move => k kbl kbh; rewrite Ha2 1:/#.
+    rewrite /set_type /zero_address.
+    by rewrite !get_setE 1..5:/#; smt(Array8.initiE).
+  + by move: (Ha2 7 _).
+  + case (_hw < _hw1) => lthw;1: by smt(sfl_size).
+    have /= := hwdec_exit _lstart i{2} _sth _ss _ps (adr2ads zero_address) (to_uint o) _ _ _ _;1..4:smt().
+    + have ->  :size (stack_increment _lstart i{2} _sth _ss _ps (adr2ads zero_address) (to_uint o)) = to_uint o by smt().
+      move : Hout'.
+      case (to_uint o < 2) => /= [|_ [ge neq]];1: smt(sfl_size size_lpathst size_ge0 size_rev count_size BS2Int.size_int2bs).
+      by smt(W32.to_uint_eq sfl_size W64.to_uint_cmp sfl_size hwinc).
+
+  + case (_hw < _hw1) => ? k *.
+    + case (k < _hw) => *. 
+      + have ? := hwinc_pathsprev i{2} _sth k _ _ _ _;1..4: smt().
+        have ? := hwinc_leaflast i{2} _sth _ _ _;1..3: smt(). 
+        by rewrite -!stack_final;smt().
+      by rewrite !H5;smt(W32.to_uint_eq sfl_size W64.to_uint_cmp stack_final).
+  + have /= := hwdec_exit  _lstart i{2} _sth _ss _ps (adr2ads zero_address) (to_uint o) _ _ _ _ _ _ _;1..6:smt(). 
+    + have ->  :size (stack_increment  _lstart i{2} _sth _ss _ps (adr2ads zero_address) (to_uint o)) = to_uint o by smt().
+      move : Hout'.
+      case (to_uint o < 2)  => /=*;1:smt().
+      by rewrite -!H5; smt(W32.to_uint_eq sfl_size W64.to_uint_cmp stack_final).
+     move => *.
+     rewrite !H5;1,2: smt(W32.to_uint_eq sfl_size W64.to_uint_cmp stack_final).
+      by smt(W32.to_uint_eq sfl_size W64.to_uint_cmp stack_final).
+
+seq 3  :
+  (#pre
+  /\ address = set_tree_index
+      (set_tree_height (set_type zero_address 2) (to_uint (nth witness heights (to_uint offset - 1)))) 
+        ((_lstart + i) %/ 2^(to_uint (nth witness heights (to_uint offset - 2)) + 1))).
++ auto => /> &hr ?????????????Ho Hs; rewrite uleE /= => H.
+  rewrite !to_uintB /=;1,2: by rewrite uleE /=; smt().
+  move => H1;rewrite H1.
+  move : (Hs (to_uint offset{hr} - 1) _);1: smt(sfl_size).
+  move : (Hs (to_uint offset{hr} - 2) _);1: smt(sfl_size).
+  move => [# Hs21 Hs22] [# Hs11 Hs12].
+
+have ? :  hw (lpathst (i{hr} + 1) _sth) <= hw (lpathst i{hr} _sth) by
+  have /= := hwinc_noentry _lstart i{hr} _sth _ss _ps (adr2ads zero_address) (to_uint offset{hr}) _; smt(sfl_size).
+
+have -> :
+     (to_uint
+         (W32.of_int (_lstart + i{hr}) `>>`
+          truncateu8 ((nth witness heights{hr} (to_uint offset{hr} - 2) + W32.one) `&` W32.of_int 31))) =
+     ((_lstart + i{hr})%/ 2^(to_uint (nth witness heights{hr} (to_uint offset{hr} - 2)) + 1)); last first.
+  + split; 1: by move => *;rewrite /set_tree_index /set_tree_height /=; smt(Array8.get_setE).
+    rewrite tP => k kb;rewrite /set_tree_index /set_tree_height /=.
+    pose x:=
+       (stack_increment _lstart i{hr} _sth _ss _ps (adr2ads zero_address) (hw (lpathst i{hr} _sth) + 1 - to_uint offset{hr})).
+    pose y := W32.of_int ((_lstart + i{hr})  %/ 2^(to_uint (nth witness heights{hr} (to_uint offset{hr} - 2)) + 1)).
+     case (0<=k<5 \/ k= 7);1:by smt(Array8.get_setE).
+     case (k=6);1:by smt(Array8.get_setE).
+     move => *; have -> : k=5 by smt().
+     rewrite !get_setE //= /#.
+
+  + rewrite /(`>>`) /= to_uint_truncateu8.
+    have -> : 31 = 2^5 - 1 by rewrite /=.
+    rewrite and_mod //= to_uintD_small /=   Hs22 /=.
+    + by have := si_heights_in_loop_bnd _lstart i{hr} _sth _ss _ps (adr2ads zero_address) (to_uint offset{hr})  (to_uint offset{hr} - 2) _ _ _;smt(h_max).
+    rewrite to_uint_shr /=;1: smt(W32.to_uint_cmp).
+    rewrite of_uintK  modz_small => /=;1: smt(l_max).
+    rewrite of_uintK  modz_small /= 1:/#.
+    rewrite modz_small 1:/#.
+    by rewrite modz_small;
+     have := si_heights_in_loop_bnd _lstart i{hr} _sth _ss _ps (adr2ads zero_address) (to_uint offset{hr})  (to_uint offset{hr} - 2) _ _ _;smt(h_max).
+
+(*
+seq 3 : (#pre
+         /\ node0 = nth nbytes_witness stack (to_uint offset - 2)
+         /\ node1 = nth nbytes_witness stack (to_uint offset - 1)
+         /\ new_node = block2bs  (trh _ps (set_tree_index (set_tree_height (set_type zero_address 2) (to_uint (nth witness heights{hr} (to_uint offset{hr} - 1))))
+                                           ((_lstart + i{hr}) %/ 2 ^ (to_uint (nth witness heights{hr} (to_uint offset{hr} - 2)) + 1)) ) (BytesToBits (NBytes.val node0) ++ BytesToBits (NBytes.val node1)))).
++ inline *; auto => /> &hr ???????????????; rewrite uleE /= => ?.
+   rewrite !to_uintB /=;1,2:by  rewrite ?uleE /=; smt().
+   move => ?.
+   rewrite /trh /thfc /= ifF. smt(@StdOrder gt0_n gt2_len).
+   rewrite /block2bs DigestBlock.insubdK. 
+   + rewrite /BytesToBits (size_flatten_ctt 8);1:smt(mapP W8.size_w2bits).
+     rewrite size_map;1: smt(NBytes.valP).
+   rewrite BytesToBitsK NBytes.valKd /rand_hash /=.
+   congr.
+
+     have Hs8 :  (size (BytesToBits (NBytes.val (nth XMSS_TreeHash.nbytes_witness stack{hr} (to_uint offset{hr} - 2)))) %/ 8) = size (chunk 8 (BytesToBits (NBytes.val (nth XMSS_TreeHash.nbytes_witness stack{hr} (to_uint offset{hr} - 2)))))     by rewrite size_chunk //.
+
+  have Hsd : (size (BytesToBits (NBytes.val (nth XMSS_TreeHash.nbytes_witness stack{hr} (to_uint offset{hr} - 2)))) +
+       size (BytesToBits (NBytes.val (nth XMSS_TreeHash.nbytes_witness stack{hr} (to_uint offset{hr} - 1))))) %/
+      8 %/ 2 = size (BytesToBits (NBytes.val (nth XMSS_TreeHash.nbytes_witness stack{hr} (to_uint offset{hr} - 2)))) %/ 8.
+        + have -> : size (BytesToBits (NBytes.val (nth XMSS_TreeHash.nbytes_witness stack{hr} (to_uint offset{hr} - 1)))) =
+            size (BytesToBits (NBytes.val (nth XMSS_TreeHash.nbytes_witness stack{hr} (to_uint offset{hr} - 2)))); last by smt().
+          rewrite /BytesToBits !(size_flatten_ctt 8);1,2: smt(mapP W8.size_w2bits). 
+          by rewrite !size_map !NBytes.valP.
+
+     have ? : size
+  (map W8.bits2w
+     (take
+        (size
+           (BytesToBits (NBytes.val (nth XMSS_TreeHash.nbytes_witness stack{hr} (to_uint offset{hr} - 2))) ++
+            BytesToBits (NBytes.val (nth XMSS_TreeHash.nbytes_witness stack{hr} (to_uint offset{hr} - 1)))) %/
+         8 %/ 2)
+        (chunk 8
+           (BytesToBits (NBytes.val (nth XMSS_TreeHash.nbytes_witness stack{hr} (to_uint offset{hr} - 2))) ++
+            BytesToBits (NBytes.val (nth XMSS_TreeHash.nbytes_witness stack{hr} (to_uint offset{hr} - 1))))))) =
+n.
+     + rewrite size_map size_cat 1:Hsd chunk_cat;1: by rewrite /BytesToBits !(size_flatten_ctt 8); smt(mapP W8.size_w2bits). 
+       rewrite Hs8  take_cat' /= take0 /= cats0 /= take_size size_chunk //. 
+       rewrite /BytesToBits !(size_flatten_ctt 8);1: smt(mapP W8.size_w2bits). 
+       by rewrite !size_map !NBytes.valP /= /#.
+
+     have ? : size
+  (map W8.bits2w
+     (drop
+        (size
+           (BytesToBits (NBytes.val (nth XMSS_TreeHash.nbytes_witness stack{hr} (to_uint offset{hr} - 2))) ++
+            BytesToBits (NBytes.val (nth XMSS_TreeHash.nbytes_witness stack{hr} (to_uint offset{hr} - 1)))) %/
+         8 %/ 2)
+        (chunk 8
+           (BytesToBits (NBytes.val (nth XMSS_TreeHash.nbytes_witness stack{hr} (to_uint offset{hr} - 2))) ++
+            BytesToBits (NBytes.val (nth XMSS_TreeHash.nbytes_witness stack{hr} (to_uint offset{hr} - 1))))))) =
+n.
+     + rewrite size_map size_cat 1:Hsd chunk_cat;1: by rewrite /BytesToBits !(size_flatten_ctt 8); smt(mapP W8.size_w2bits). 
+       rewrite Hs8  drop_cat /= drop0 /= /BytesToBits flattenK //;1:smt(mapP W8.size_w2bits). 
+       by rewrite !size_map !NBytes.valP /= /#.
+
+congr;congr;congr;1,4..:by rewrite /prf.
+
+   + rewrite /BitsToBytes size_map size_chunk // -map_take.
+     rewrite NBytes.insubdK 1:/# map_take size_cat Hsd.
+     rewrite chunk_cat;1:by rewrite /BytesToBits !(size_flatten_ctt 8); smt(mapP W8.size_w2bits). 
+     rewrite map_cat Hs8 -(size_map W8.bits2w) take_cat' /= take0 cats0 take_size.
+     have ->: map W8.bits2w
+  (chunk 8 (BytesToBits (NBytes.val (nth XMSS_TreeHash.nbytes_witness stack{hr} (to_uint offset{hr} - 2))))) =
+     BitsToBytes (BytesToBits (NBytes.val (nth XMSS_TreeHash.nbytes_witness stack{hr} (to_uint offset{hr} - 2)))) by smt().
+     by rewrite BytesToBitsK.
+
+   + rewrite /BitsToBytes size_map size_chunk // -map_drop.
+     rewrite NBytes.insubdK 1:/# map_drop size_cat Hsd.
+     rewrite chunk_cat;1:by rewrite /BytesToBits !(size_flatten_ctt 8); smt(mapP W8.size_w2bits). 
+     rewrite map_cat Hs8 -(size_map W8.bits2w) drop_cat /= drop0 /=. 
+     have ->: map W8.bits2w
+  (chunk 8 (BytesToBits (NBytes.val (nth XMSS_TreeHash.nbytes_witness stack{hr} (to_uint offset{hr} - 1))))) =
+     BitsToBytes (BytesToBits (NBytes.val (nth XMSS_TreeHash.nbytes_witness stack{hr} (to_uint offset{hr} - 1)))) by smt().
+     by rewrite BytesToBitsK.
+*)
++ auto => /> &hr ?????????????Ho Hs; rewrite uleE /= => H.
+  rewrite !to_uintB /=;1..2,4: by rewrite uleE /=; smt().
+  + by rewrite uleE /= to_uintB /=; rewrite ?uleE /=; smt().
+
+  move => H1;rewrite H1.
+  move : (Hs (to_uint offset{hr} - 1) _);1: smt(sfl_size).
+  move : (Hs (to_uint offset{hr} - 2) _);1: smt(sfl_size).
+  move => [# Hs21 Hs22] [# Hs11 Hs12].
+
+have ? :  hw (lpathst (i{hr} + 1) _sth) <= hw (lpathst i{hr} _sth) by
+  have /= := hwinc_noentry _lstart i{hr} _sth _ss _ps (adr2ads zero_address) (to_uint offset{hr}) _; by smt(sfl_size).
+
+(*
+have ? :  hw (lpathst _lstart (i{hr} + 1) _sth) <= hw (lpathst _lstart i{hr} _sth) by
+ have /=:= hwinc_noentry _lstart i{hr} _sth _ss _ps _ad (to_uint offset{hr}) _;smt().
+*)
+split;1: smt().
+
+have Hsil := si_size_in_loop _lstart i{hr} _sth _ss _ps (adr2ads zero_address) (to_uint offset{hr}) _ _ _ _ _ _ _ _; 1..8: smt().
+
+  do split.
+  + move => *;split;2:smt().
+    rewrite Ho.
+    rewrite Ho /stack_increment /= ifF 1:/# ifF 1:/# /= !size_cat /=.
+    rewrite size_take;1:smt(size_ge0).
+    by  smt(sfl_size size_take).
+  + by smt(size_put).
+  + by smt(size_put).
+  + rewrite Ho /stack_increment /= ifF 1:/# /= !size_cat /=.
+    rewrite size_take;1:smt(size_ge0).
+    have -> /= : !(hw (lpathst i{hr} _sth) < hw (lpathst (i{hr} + 1) _sth)) by smt().
+    by case (to_uint offset{hr} - 1 < size (stack_from_leaf _lstart i{hr} _sth _ss _ps (adr2ads zero_address)));rewrite size_cat /=; by  smt(sfl_size size_take).
+
+  + move => k kbl kbh.
+    rewrite !nth_put;1,2: smt(size_lpathst count_size BS2Int.size_int2bs size_rev).
+    have kbh1 : k < to_uint offset{hr} -1.
+    + move : kbh;rewrite /stack_increment /= ifF 1:/# size_cat /=.
+      smt(size_take sfl_size).
+    case (to_uint offset{hr} - 2 = k) => Hk; last first.
+    + rewrite !Hs; 1,2: smt().
+      rewrite /stack_increment /= ifF 1:/#.
+      have -> /= : !(hw (lpathst i{hr} _sth) < hw (lpathst (i{hr} + 1) _sth)) by smt().
+      rewrite !nth_cat /= ifT;1:smt(size_take sfl_size size_ge0).
+      have  /=: !(k - size (take (to_uint offset{hr} - 2) (stack_from_leaf _lstart i{hr} _sth _ss _ps (adr2ads zero_address))) = 0) by smt(sfl_size size_take).
+      rewrite !ifT;1:smt(size_take sfl_size size_ge0).
+      by rewrite !nth_take;smt(size_take sfl_size size_ge0).
+   split.
+  + (*rewrite /bs2block /block2bs. NBytes.insubdK;1: 
+      by rewrite /BitsToBytes size_map size_chunk 1:/# DigestBlock.valP /#. 
+    rewrite BitsToBytesK;1: by rewrite DigestBlock.valP /=; smt().
+    rewrite DigestBlock.valKd /=.*)
+    have /= := si_reduced_node _lstart i{hr} _sth _ss _ps (adr2ads zero_address) (to_uint offset{hr}) _ _ _ _ _ _ _;1..7:smt().
+
+    rewrite Hk => -> @/trh /=.
+    rewrite ifF; 1: smt(ge1_n).
+    rewrite /bs2block. do 4! congr.
+    rewrite -Hs12 H1 Hk.
+    rewrite zeroadsE /set_typeidx (HAX.Adrs.insubdK _ zeroadiP) /put /=.
+    rewrite /set_thtbidx (HAX.Adrs.insubdK [0; 0; 0; trhtype]) 1:/#.
+    rewrite /put /= HAX.Adrs.insubdK /valid_adrsidxs /= /valid_xidxvalslp /valid_xidxvalslptrh /=.
+    right; right. rewrite /valid_tbidx /valid_thidx /nr_nodes.
+    rewrite divz_ge0 1:expr_gt0 1:// /trhtype /=.
+    have ? : 0 <= to_uint (nth witness heights{hr} k) < h by 
+      smt(si_heights_in_loop_bnd).
+    split; 2:smt(). 
+    split; 1: smt().
+    + move => *.
+      apply (ler_lt_trans (2^h %/ 2 ^ (to_uint (nth witness heights{hr} k) + 1)));  1:  by  apply leq_div2r; 1,2:smt(expr_ge0).  
+      rewrite -exprD_subz 1,2:/#; apply gt_exprsbde; smt(). 
+    rewrite /idxs2adr /set_tree_index /set_tree_height /set_type.
+    rewrite tP => ii rngi; rewrite initE rngi /= ?get_setE 1..7://.
+    rewrite initE.
+    case (ii = 0) => [-> //|].
+    case (ii = 1) => [-> //|].
+    case (ii = 2) => [-> //|].
+    case (ii = 3) => [-> //|].
+    case (ii = 4) => [-> //|].
+    by case (ii = 5) => [-> //| /#].	(* FIXME: WTF is my smt, why does it only solve from here? and not above as `rewrite initE /#`? *)
+    rewrite take_cat DigestBlock.valP /= take0 cats0 /=.
+    rewrite -Hk -Hs21 /bs2block DigestBlock.insubdK.
+    rewrite /BytesToBits (: n = size (map W8.w2bits (NBytes.val (nth witness stack{hr} (to_uint offset{hr} - 2))))).
+    + by rewrite size_map NBytes.valP.
+    by rewrite -size_flatten_ctt 2:// => x /mapP [xx [_ ->]]; rewrite size_w2bits.
+    rewrite BytesToBitsK NBytes.valKd.
+    + apply nth_change_dfl;split => *;1:smt().
+      have : to_uint offset{hr} <= hw (lpathst i{hr} _sth) + 1 by smt().
+      by smt( hw_le_size size_drop size_lpathst).
+    rewrite -Hs 1:/#.
+    rewrite drop_cat DigestBlock.valP /= drop0 -Hs 1:/# DigestBlock.insubdK.
+    + rewrite /BytesToBits (: n = size (map W8.w2bits (NBytes.val (nth witness stack{hr} (to_uint offset{hr} - 1))))).
+      + by rewrite size_map NBytes.valP.
+      by rewrite -size_flatten_ctt 2:// => x /mapP [xx [_ ->]]; rewrite size_w2bits.
+    rewrite BytesToBitsK NBytes.valKd.
+    apply nth_change_dfl;split => *;1:smt().
+    have : to_uint offset{hr} <= hw (lpathst i{hr} _sth) + 1 by smt().
+    by smt( hw_le_size size_drop size_lpathst).
+ rewrite to_uintD_small /=.
+ + rewrite Hs22.
+   + have := si_heights_in_loop_bnd _lstart i{hr} _sth _ss _ps (adr2ads zero_address) (to_uint offset{hr}) (to_uint offset{hr} - 2) _ _ _ _ _ _ _ _;smt(h_max).
+     rewrite Hs22.
+     rewrite /stack_increment /= ifF 1:/# nth_cat /=.
+     have -> /= : !(hw (lpathst i{hr} _sth) < hw (lpathst (i{hr} + 1) _sth)) by smt().
+     rewrite !nth_cat /= ifT;1:smt(size_take sfl_size size_ge0).
+     rewrite ifF;1:smt(size_take sfl_size size_ge0).
+     rewrite ifT;1:smt(size_take sfl_size size_ge0).
+     rewrite ifF;1:smt(size_take sfl_size size_ge0).
+     rewrite /node_from_path /=.
+     smt(nth_take).
+qed.
+
+op pkrel (pks : pkXMSSTWRFC) (pkr : xmss_pk) : bool =
+  pks.`1 = bs2block pkr.`pk_root /\ pks.`2 = pkr.`pk_pub_seed.
+
+op skrel (sks : skXMSSTWRFC) (skr : xmss_sk) : bool =
+     sks.`1 = skr.`sk_prf
+  /\ Index.val sks.`2.`1 = to_uint skr.`idx
+  /\ sks.`2.`2 = skr.`sk_seed
+  /\ sks.`2.`3.`1 = bs2block skr.`sk_root
+  /\ sks.`2.`3.`2 = skr.`pub_seed_sk.
+
+
+module RFC_O (O : DSS_RFC.RO.POracle) = {
+  proc o(xm : threen_bytes * W8.t list) : nbytes  = {
+    var x : threen_bytes;
+    var m : W8.t list;
+    var xs : W8.t list list;
+    var mk : nbytes;
+    var root : dgstblock;
+    var idx : index;
+    var cm : dgstblock;
+
+    (x, m) <- xm;
+    xs <- chunk n (ThreeNBytesBytes.val x);
+
+    mk <- NBytes.insubd (nth witness xs 0);
+    root <- DigestBlock.insubd (BytesToBits (nth witness xs 1));
+    idx <- Index.insubd (BS2Int.bs2int (BytesToBits (nth witness xs 2)));
+
+    cm <@ O.o(mk, (root, idx, m));
+
+    return NBytes.insubd (BitsToBytes (DigestBlock.val cm));
+  }
+}.
+
+equiv kg_eq (O <: DSS_RFC.RO.POracle) :
+  XMSS_TW_RFC(O).keygen ~ XMSS_RFC_Abs(RFC_O(O)).kg :
+    ={arg} ==> pkrel res{1}.`1 res{2}.`2 /\ skrel res{1}.`2 res{2}.`1.
+proof.
+have ? := h_g0; have ? := expr_gt0.
+
+proc.
+inline {1} keygen.
+inline{2} sample_randomness.
+swap {2} [5..7] -4. swap {2} 2 -1; seq 3 3 : (NBytes.val ss{1} = sk_seed0{2} /\ NBytes.val ms{1} = sk_prf0{2} /\ NBytes.val ps{1} = pub_seed0{2}).
++ do 3!(rnd NBytes.val NBytes.insubd); auto => />.
+   have H := supp_dlist W8.dword n.
+   have Hn:= ge1_n.
+   split => *; 1: smt(NBytes.insubdK ge1_n supp_dlist).
+   split => *;1: (rewrite dmapE; apply mu_eq_support => x Hx;smt(NBytes.valK)).
+   split => *;1:smt(NBytes.valP supp_dmap).
+   split => *;1: smt(NBytes.insubdK NBytes.valK ge1_n supp_dlist).
+   smt(NBytes.valP supp_dmap).
+
+sp;wp => /=. conseq
+    (: _ ==> (val_bt_trh (list2tree leafl{1}) ps{1} (set_typeidx (XAddress.val adc) trhtype) h 0 =
+              DigestBlock.insubd (BytesToBits (NBytes.val root{2})))).
++ auto => /> &1 *; smt(NBytes.valK Index.insubdK).
+
+ecall {1} (leaves_correct  ps0{1} ss0{1} ad{1}) => /=.
+ecall {2} (tree_hash_correct pub_seed{2} sk_seed{2} 0 h).
+auto => /> &1;do split.
++ rewrite /set_layer_addr /zero_address /= tP => *;  smt(Array8.get_setE Array8.initiE).
++ smt(h_g0).
+
+move=> ??? rr ->.
+suff @/adc ->: XAddress.val (XAddress.insubd (HAX.Adrs.insubd (adr2idxs zero_address))) = adr2ads zero_address.
++ by smt(NBytes.valK).
+by rewrite XAddress.insubdK /valid_xadrs; smt(HAX.Adrs.valP take_size).
+qed.
+
+
+(*
+op skrel(ask : skXMSSTW, sk : xmss_sk) =
+   ask.`1 = sk.`sk_prf /\
+   Index.val ask.`2.`1 = to_uint sk.`idx /\ 0 <= Index.val ask.`2.`1 <= 2^h /\
+   ask.`2.`2 = sk.`sk_seed  /\
+   ask.`2.`3 = sk.`pub_seed_sk
+   (* ask.`2.`4 = ??? Why is the address in/not in the sk/pk? *)
+   (* ??? = sk.`pk_root Why is the root not in/in the sk? *).
+
+op pkrel(apk : pkXMSSTW, pk : xmss_pk) =
+   apk.`1 = DigestBlock.insubd (BytesToBits (NBytes.val pk.`pk_root)) /\
+   apk.`2 = pk.`pk_pub_seed
+   (* apk.`3 = ??? Why is the address in the sk/pk? *)
+   (* ??? = pk.`pk_oid I guess abstract proofs fon't care about oid *).
+*)
+
+
+(*
+(* FD + WR *)
+equiv kg_eq : XMSS_TW(FakeRO).keygen ~ XMSS_PRF.kg :
+  ={arg} ==> pkrel res{1}.`1 res{2}.`2 /\ skrel res{1}.`2 res{2}.`1.
+proof.
+have ? := h_g0; have ? := expr_gt0.
+proc. inline {1} 2. inline {1} 5. inline {2} 5.
+swap {2} [5..7] -4. swap {2} 2 -1; seq 3 3 : (NBytes.val ss{1} = sk_seed0{2} /\ NBytes.val ms{1} = sk_prf0{2} /\ NBytes.val ps{1} = pub_seed0{2}).
++ do 3!(rnd NBytes.val NBytes.insubd); auto => />.
+   have H := supp_dlist W8.dword n.
+   have Hn:= Params.ge0_n.
+   split => *;1: smt(NBytes.insubdK NBytes.valK Params.ge0_n supp_dlist).
+   split => *;1: (rewrite dmapE; apply mu_eq_support => x Hx;smt(NBytes.valK)).
+   split => *;1:smt(NBytes.valP supp_dmap).
+   split => *;1: smt(NBytes.insubdK NBytes.valK Params.ge0_n supp_dlist).
+   smt(NBytes.valP supp_dmap).
+
+sp;wp => /=. conseq 
+    (: _ ==> (val_bt_trh (list2tree leafl{1}) ps{1} (set_typeidx (XAddress.val witness) trhtype) h 0 =
+              DigestBlock.insubd (BytesToBits (NBytes.val root{2})))).
++ auto => /> &1 *; smt(NBytes.valK Index.insubdK). 
+
+ecall {1} (leaves_correct  ps0{1} ss0{1} ad{1}) => /=.
+ecall {2} (tree_hash_correct pub_seed{2} sk_seed{2} 0 h address{2}).
+auto => /> &1;do split. 
++ rewrite /set_layer_addr /zero_address /= tP => *;  smt(Array8.get_setE Array8.initiE).  
++ smt(h_g0).
+move=> -> ?? rr ->;congr;1:smt(NBytes.valK).
+rewrite /set_typeidx;congr.
+apply (eq_from_nth witness);rewrite !size_put;1: smt(HAX.Adrs.valP).
+by move => i ib;rewrite !(nth_put);smt(size_put HAX.Adrs.valP).
+qed.
+*)
+
+
+(* Signature type is abused with two index copies because I need this to simulate
+   the actual operation of the implementation *)
+
+op sigrel(asig : sigXMSSTW, sig : sig_t) =
+   asig.`1 = sig.`r /\
+   Index.val asig.`2.`1 = to_uint sig.`sig_idx /\
+   asig.`2.`2 = DBLL.insubd
+     (map (fun (b : nbytes) => DigestBlock.insubd (BytesToBits (NBytes.val b))) (LenNBytes.val sig.`r_sig.`1)) /\
+   asig.`2.`3 = DBHL.insubd
+     (map (fun (b : nbytes) => DigestBlock.insubd (BytesToBits (NBytes.val b))) (AuthPath.val sig.`r_sig.`2)).
+
+
+(*
+op sigrel(asig : sigXMSSTW, sig : sig_t) =
+   asig.`1.`1 = sig.`r /\
+   asig.`1.`2 = to_uint sig.`sig_idx /\
+   Index.val asig.`2.`1 = to_uint sig.`sig_idx /\ 0 <= Index.val asig.`2.`1 <= 2^h /\
+   asig.`2.`2 = DBLL.insubd
+     (map (fun (b : nbytes) => DigestBlock.insubd (BytesToBits (NBytes.val b))) (LenNBytes.val sig.`r_sig.`1)) /\
+   asig.`2.`3 = DBHL.insubd
+     (map (fun (b : nbytes) => DigestBlock.insubd (BytesToBits (NBytes.val b))) (AuthPath.val sig.`r_sig.`2)).
+*)
+
+(*
+(* FD + WR : FIXME : THERE IS SOMETHING WRONG IN THE DEFINITION OF INSUBD FOR INDEX *)
+equiv sig_eq : XMSS_TW(FakeRO).sign ~ XMSS_PRF.sign : skrel sk{1} sk{2} /\ ={m} /\ Index.val sk{1}.`2.`1 < 2^h -1  ==>
+   sigrel res{1}.`1 res{2}.`1 /\ skrel res{1}.`2 res{2}.`2.
+proof.
+proc. inline {1} 6. inline {1} 8. inline {1} 5.
+swap {1} 21 -4. swap {1} [13..17] -1. swap {1} [11..16] -1. swap {1} [9..15] -6. inline {2} 7. inline {2} 16.
+
+wp 20 25. 
+sp 8 3 => /=.  
+seq 1 1 : (skrel (ms{1},sk1{1}) sk{2} 
+        /\ ={m} 
+        /\ 0 <= Index.val idx0{1} < 2 ^ h
+        /\ Index.val idx0{1} = to_uint idx{2}
+        /\ sk_prf{2} = sk{2}.`Types.sk_prf 
+        /\ Index.val skfl{1}.`1 = to_uint idx{2}).
++ auto => /> &1 &2 *;do split. 
+  + rewrite Index.insubdK 1:/# to_uintD_small;smt(pow2_32 expr_ge0 h_max gt_exprsbde h_g0).
+  + smt(Index.valP).
+  + move => *;rewrite Index.insubdK /#. 
+  + smt().
+
+sp;conseq => />. 
+
+seq 1 0 : #pre. admit.  (* we need to meta-swap this *)
+
+seq 2 1 : (#pre /\ ap{1} =
+   DBHL.insubd
+     (map (fun (b : Params.nbytes) => DigestBlock.insubd (BytesToBits (NBytes.val b))) (AuthPath.val auth0{2}))); last first.  
+
++ seq 0 3 : (#pre /\ sigWOTS{1} =
+   DBLL.insubd
+     (map (fun (b : Params.nbytes) => DigestBlock.insubd (BytesToBits (NBytes.val b))) (LenNBytes.val sig_ots{2}))). admit.  (* we need to meta-swap this *)
+
+
+   auto => /> &1 &2; rewrite /mkg => />  *; split;2:smt().
+ + congr; congr.
+   + by congr;rewrite /W64toBytes_ext /toByte_64 //.
+   + rewrite NBytes.insubdK /toByte.
+     + rewrite size_rev size_mkseq; smt(gt0_n). 
+   + congr.  
+     + congr => /=;congr;congr;congr. 
+       + apply W32.to_uint_eq=> /=; rewrite of_uintK /=.
+         by rewrite modz_small /=;smt(pow2_32 expr_ge0 h_max gt_exprsbde h_g0).
+
+inline {2} 1. wp; conseq />.
+ecall {1} (leaves_correct  ps{1} ss{1} ad{1}) => /> /=.
+swap {2} [6..7] -5; seq 0 2: (#pre /\ size authentication_path{2} = h); 1: by auto => />;smt(size_nseq h_g0). 
+sp 0 4.
+
+while {2} (#pre /\ 0 <= j{2} <= h /\ forall kk, 0 <= kk < j{2} => 
+        nth witness (map (fun (b : Params.nbytes) => DigestBlock.insubd (BytesToBits (NBytes.val b)))
+       (AuthPath.val (AuthPath.insubd authentication_path{2}))) kk =
+    nth witness (DBHL.val (cons_ap_trh
+    (list2tree
+       (map
+          (leafnode_from_idx (NBytes.insubd (NBytes.val ss{1})) (NBytes.insubd (NBytes.val ps{1}))
+             (set_layer_addr zero_address 0)) (range 0 (2 ^ h)))) idx0{1} ps{1} (
+    set_typeidx ad{1} 2))) kk) (h - j{2});last first. 
++ auto => /> &1 &2 *;split;1: smt(h_g0).
+  move => ap2 j2;do split;1:smt().
+  move => ? <-?? H. 
+  rewrite -DBHL.valKd;congr.
+  apply (eq_from_nth witness);1: smt(DBHL.valP size_map AuthPath.valP).
+  move => k kb.
+  rewrite  (H k _);1:smt(DBHL.valP size_map AuthPath.valP).
+  by smt().
+
+move => &1 ?. 
+sp;wp. 
+exlim pub_seed0, sk_seed0,  (k * 2 ^ j), j,  address1 => _ps _ss _start _sth _ad. 
+call (tree_hash_correct _ps _ss _start _sth _ad).
+auto => /> &2 ?????????????H?;do split. 
++ smt(W32.to_uint_cmp StdOrder.IntOrder.expr_ge0).
++ move => *.
+  pose xx := to_uint ((idx{2} `>>` W8.of_int _sth) `^` W32.one).
+  have -> :  xx =
+            if (to_uint idx{2} %/ 2^_sth) %% 2 = 0 
+            then (to_uint idx{2} %/ 2^_sth) + 1  
+            else (to_uint idx{2} %/ 2^_sth) - 1 by admit. (* xor 1 over integers *)
+  case (to_uint idx{2} %/ 2^ _sth %% 2 = 0) => He.
+  + have ? : to_uint idx{2} + 2*2^_sth < 2^h. admit. (* adding a missing bit *)
+    rewrite mulrDl /= divzE.  smt(@StdOrder).
+  + rewrite mulrDl /= divzE /=.  smt(@StdOrder).
+  + smt(@IntDiv).
+move => ???rr Hrr; do split. 
++ smt(size_put).
++ smt().
++ smt().
++ move => k *. 
+  rewrite (nth_map witness) /=;1:smt(AuthPath.valP). 
+  rewrite AuthPath.insubdK;1:smt(size_put).
+  rewrite nth_put 1:/#. 
+  case (k = _sth) => Hk.
+  + rewrite Hk /= Hrr /cons_ap_trh DBHL.insubdK.
+    + admit. (* properties of functional ap operators *)
+    + admit. (* properties of functional ap operators *)
+  + rewrite ifF 1:/# /=. 
+    rewrite -H 1:/# (nth_map witness) /=;smt(AuthPath.valP AuthPath.insubdK). 
++ smt().
+qed.
+*)
+
+equiv sig_eq (O <: DSS_RFC.RO.POracle) :
+  XMSS_TW_RFC(O).sign ~ XMSS_RFC_Abs(RFC_O(O)).sign :
+  ={glob O} /\ skrel sk{1} sk{2} /\ ={m} /\ Index.val sk{1}.`2.`1 < 2^h -1  ==>
+     sigrel res{1}.`1 res{2}.`1 /\ skrel res{1}.`2 res{2}.`2.
+proof.
+proc.
+inline{1} RFC.FL_XMSS_TW_RFC.sign.
+inline{1} FL_XMSS_TW_ES.sign.
+inline{2} treesig.
+swap{1} 15 2.
+swap{1} ^m0<- -1.
+swap{1} ^m1<- -2.
+swap{1} [^sk0<- .. ^ad<-] -3.
+swap{2} [^sk0<- .. ^pub_seed<-] -2.
+sp.
+wp 17 20 => />.
+elim*=> skt.
+seq 1 1 : (#pre /\ cm{1} = bs2block _M'{2}).
++ inline{2} *.
+  wp; sp.
+  call (: true).
+  skip => &1 /> *.
+  do ? split.
+  + admit.
+  + admit.
+  + admit.
+  move => 3? m.
+  rewrite /bs2block.
+  admit.
+sp.
+seq 2 1 : (   #pre
+           /\ ap{1}
+              =
+              DBHL.insubd
+              (map (fun (b : nbytes) => bs2block b) (AuthPath.val auth0{2}))).
++ wp; ecall{1} (leaves_correct ps{1} ss{1} ad{1}).
+  inline{2} buildAuthPath.
+  sp 0 4; wp => /=.
+  while{2} (   #pre
+            /\ size authentication_path{2} = h
+            /\ 0 <= j{2} <= h
+            /\ (forall kk, 0 <= kk < j{2} =>
+                 nth witness (DBHL.val (DBHL.insubd (map (fun (b : nbytes) => bs2block b)
+                                                     (AuthPath.val (AuthPath.insubd authentication_path{2}))))) kk
+                 =
+                 nth witness (DBHL.val
+                              (cons_ap_trh
+                               (list2tree (map (leafnode_from_idx ss{1} ps{1} (adr2ads (set_layer_addr zero_address 0))) (range 0 (2 ^ h))))
+                               idx0{1} ps{1} (set_typeidx ad{1} 2))) kk))
+             (h - j{2}); last first.
+  + auto => &1 &2 />.
+    move=> *. split.  smt(size_nseq h_g0).
+    move=> apt jt; split; 1: smt().
+    move=> 4? eqnth.
+    apply /DBHL.val_inj /(eq_from_nth witness); 1: smt(DBHL.valP).
+    rewrite DBHL.valP => i rng_i.
+    rewrite ?NBytes.valKd eqnth 1:/#; do 6! congr.
+    admit.
+  auto.
+  sp.
+  exlim pub_seed0, sk_seed0,  (k * 2 ^ j), j, address1 => _ps _ss _start _sth _ad.
+  call (tree_hash_correct _ps _ss _start _sth).
+  auto => &2 />.
+  move=> 9? eqnth ?; split.
+  + admit.
+  move=> 3? rr rval; split; 2: smt().
+  split; 1: smt(size_put).
+  split; 1: smt(size_put).
+  move=> kk g0k ltj1k.
+  case (kk < j{2}) => kkj.
+  + rewrite -eqnth 1:/#.
+    admit.
+  rewrite (: kk = j{2}) 1:/#.
+  rewrite AuthPath.insubdK 2:DBHL.insubdK 3:(nth_map witness); 1..3: smt(size_map size_put).
+  rewrite nth_put 1:/# /= /bs2block rval.
+  admit.
+sp; elim*=> adt.
+seq 1 1 : (   #pre
+           /\ sigWOTS{1}
+              =
+              DBLL.insubd (map (fun (b : nbytes) => bs2block b) (LenNBytes.val sig_ots{2}))).
++ inline{1} WOTS_TW_ES.sign; inline{2} WOTS.sign_seed.
+  wp.
+  while (   ps0{1} = pub_seed0{2}
+         /\ ad0{1} = adr2ads address1{2}
+         /\ map BaseW.val (EmsgWOTS.val em{1}) = msg{2}
+         /\ DBLL.val skWOTS0{1} = map bs2block (LenNBytes.val wots_skey{2})
+         /\ (forall j, 0 <= j < size sig2{1} =>
+             nth witness sig2{1} j = bs2block (nth witness sig0{2} j))
+         /\ size sig2{1} = i{2}
+         /\ size sig2{1} <= XMSS_Security.FLXMSSTW.len).
+  + admit.
+  admit.
+auto => &1 &2 /> ? eqv *.
+rewrite Index.insubdK; 1:smt(Index.valP).
+by rewrite /RFC.skr2sko /= eqv /= to_uintD_small; smt(pow2_32 expr_ge0 h_max gt_exprsbde h_g0).
+(*
+inline{2} WOTS.checksum.
+swap {1} 22 -4.
+swap {1} [14..18] -1.
+swap {1} [11..16] -1.
+swap {1} [9..15] -6.
+inline {2} 7. inline {2} 16.
+
+wp 20 25.
+sp 8 3 => /=.
+seq 1 1 : (skrel (ms{1},sk1{1}) sk{2}
+        /\ ={m}
+        /\ Index.val idx0{1} = to_uint idx{2}
+        /\ sk_prf{2} = sk{2}.`sk_prf
+        /\ Index.val skfl{1}.`1 = to_uint idx{2}).
++ auto => /> &1 &2 *;do split.
+  + rewrite Index.insubdK 1:/# to_uintD_small;smt(pow2_32 expr_ge0 h_max gt_exprsbde h_g0).
+  + smt(Index.valP).
+  + move => *;rewrite Index.insubdK /#.
+  + smt().
+
+sp;conseq => />.
+
+seq 1 0 : #pre. admit.  (* we need to meta-swap this *)
+
+seq 2 1 : (#pre /\ ap{1} =
+   DBHL.insubd
+     (map (fun (b : Params.nbytes) => DigestBlock.insubd (BytesToBits (NBytes.val b))) (AuthPath.val auth0{2}))); last first.  
+
++ seq 0 3 : (#pre /\ sigWOTS{1} =
+   DBLL.insubd
+     (map (fun (b : Params.nbytes) => DigestBlock.insubd (BytesToBits (NBytes.val b))) (LenNBytes.val sig_ots{2}))). admit.  (* we need to meta-swap this *)
+
+
+   auto => /> &1 &2; rewrite /mkg => />  *; split;2:smt().
+ + congr; congr.
+   + by congr;rewrite /W64toBytes_ext /toByte_64 //.
+   + rewrite NBytes.insubdK /toByte.
+     + rewrite size_rev size_mkseq; smt(gt0_n). 
+   + congr.  
+     + congr => /=;congr;congr;congr. 
+       + apply W32.to_uint_eq=> /=; rewrite of_uintK /=.
+         by rewrite modz_small /=;smt(pow2_32 expr_ge0 h_max gt_exprsbde h_g0).
+
+inline {2} 1. wp; conseq />.
+ecall {1} (leaves_correct  ps{1} ss{1} ad{1}) => /> /=.
+swap {2} [6..7] -5; seq 0 2: (#pre /\ size authentication_path{2} = h); 1: by auto => />;smt(size_nseq h_g0). 
+sp 0 4.
+
+while {2} (#pre /\ 0 <= j{2} <= h /\ forall kk, 0 <= kk < j{2} => 
+        nth witness (map (fun (b : Params.nbytes) => DigestBlock.insubd (BytesToBits (NBytes.val b)))
+       (AuthPath.val (AuthPath.insubd authentication_path{2}))) kk =
+    nth witness (DBHL.val (cons_ap_trh
+    (list2tree
+       (map
+          (leafnode_from_idx (NBytes.insubd (NBytes.val ss{1})) (NBytes.insubd (NBytes.val ps{1}))
+             (set_layer_addr zero_address 0)) (range 0 (2 ^ h)))) idx0{1} ps{1} (
+    set_typeidx ad{1} 2))) kk) (h - j{2});last first. 
++ auto => /> &1 &2 *;split;1: smt(h_g0).
+  move => ap2 j2;do split;1:smt().
+  move => ? <-?? H. 
+  rewrite -DBHL.valKd;congr.
+  apply (eq_from_nth witness);1: smt(DBHL.valP size_map AuthPath.valP).
+  move => k kb.
+  rewrite  (H k _);1:smt(DBHL.valP size_map AuthPath.valP).
+  by smt().
+
+move => &1 ?. 
+sp;wp. 
+exlim pub_seed0, sk_seed0,  (k * 2 ^ j), j,  address1 => _ps _ss _start _sth _ad. 
+call (tree_hash_correct _ps _ss _start _sth _ad).
+auto => /> &2 ?????????????H?;do split. 
++ smt(W32.to_uint_cmp StdOrder.IntOrder.expr_ge0).
++ move => *.
+  pose xx := to_uint ((idx{2} `>>` W8.of_int _sth) `^` W32.one).
+  have -> :  xx =
+            if (to_uint idx{2} %/ 2^_sth) %% 2 = 0 
+            then (to_uint idx{2} %/ 2^_sth) + 1  
+            else (to_uint idx{2} %/ 2^_sth) - 1 by admit. (* xor 1 over integers *)
+  case (to_uint idx{2} %/ 2^ _sth %% 2 = 0) => He.
+  + have ? : to_uint idx{2} + 2*2^_sth < 2^h. admit. (* adding a missing bit *)
+    rewrite mulrDl /= divzE.  smt(@StdOrder).
+  + rewrite mulrDl /= divzE /=.  smt(@StdOrder).
+  + smt(@IntDiv).
+move => ???rr Hrr; do split. 
++ smt(size_put).
++ smt().
++ smt().
++ move => k *. 
+  rewrite (nth_map witness) /=;1:smt(AuthPath.valP). 
+  rewrite AuthPath.insubdK;1:smt(size_put).
+  rewrite nth_put 1:/#. 
+  case (k = _sth) => Hk.
+  + rewrite Hk /= Hrr /cons_ap_trh DBHL.insubdK.
+    + admit. (* properties of functional ap operators *)
+    + admit. (* properties of functional ap operators *)
+  + rewrite ifF 1:/# /=. 
+    rewrite -H 1:/# (nth_map witness) /=;smt(AuthPath.valP AuthPath.insubdK). 
++ smt().
+*)
+qed.
+
+equiv ver_eq (O <: DSS_RFC.RO.POracle) :
+  XMSS_TW_RFC(O).verify ~ XMSS_RFC_Abs(RFC_O(O)).verify :
+    pkrel pk{1} pk{2} /\ ={m, glob O} /\ sigrel sig{1} s{2}
+  ==>
+    ={res}.
+proof.
+proc.
+seq 5 9 : (   pkrel pk{1} pk{2}
+           /\ to_uint idx_sig{2} < l
+           /\ Index.val sigfl{1}.`1 = to_uint idx_sig{2}
+           /\ (map DigestBlock.val (DBLL.val sigfl{1}.`2)) = map (BytesToBits \o NBytes.val) (LenNBytes.val sig_ots{2})
+           /\ (map DigestBlock.val (DBHL.val sigfl{1}.`3) = map (BytesToBits \o NBytes.val) (AuthPath.val auth{2}))
+           /\ DigestBlock.val cm{1} = BytesToBits (NBytes.val _M'{2})
+           /\ address{2} = zero_address
+           /\ DigestBlock.val pk{1}.`1 = BytesToBits (NBytes.val root{2})
+           /\ pk{1}.`2 = _seed{2}
+           /\ root{2} = pk{2}.`pk_root).
++ inline{2} 9.
+  wp; call (_: true).
+  auto=> &1 &2 /> *.
+  admit.
+wp; inline{1} verify; inline{1} root_from_sigFLXMSSTW; inline{2} rootFromSig.
+sp; seq 1 1 : (   #pre
+               /\ map DigestBlock.val (DBLL.val pkWOTS0{1}) =  map (BytesToBits \o NBytes.val) (LenNBytes.val pk_ots{2})).
++ admit.
+wp; sp 0 5; elim* => ad2.
+exlim nodes0{2} => lf2.
+while{2} (BytesToBits (NBytes.val nodes0{2})
+          =
+          (let app = drop (h - k{2}) (map bs2block (AuthPath.val auth0{2})) in
+           let idp = (rev (BS2Int.int2bs k{2} (to_uint idx_sig0{2}))) in
+           let lfp = bs2block lf2 in
+           DigestBlock.val (val_ap_trh_gen app idp lfp _seed0{2} (adr2ads ad2) k{2} (to_uint idx_sig0{2} %/ 2 ^ k{2})))
+          /\ 0 <= k{2} <= h)
+         (h - k{2}).
++ move => _ z.
+  proc change 2 : (! odd (to_uint idx_sig0 %/ 2 ^ k)).
+  + admit.
+  auto => &1 &2 />.
+  admit.
+auto => &1 &2 />.
+admit.
+qed.
+(* PY *)
+(*
+equiv ver_eq : XMSS_TW(FakeRO).verify ~ XMSS_PRF.verify :
+       pkrel pk{1} pk{2} /\ ={m} /\ sigrel sig{1} s{2}
+    /\ to_uint s{2}.`sig_idx < l
+  ==>
+    ={res}.
+proof.
+proc=> /=.
+inline{1} 3.
+seq 6 9 : (   pkrel pk{1} pk{2}
+           /\ to_uint idx_sig{2} < l
+           /\ Index.val sigfl{1}.`1 = to_uint idx_sig{2}
+           /\ (map DigestBlock.val (DBLL.val sigfl{1}.`2)) = map (BytesToBits \o NBytes.val) (LenNBytes.val sig_ots{2})
+           /\ (map DigestBlock.val (DBHL.val sigfl{1}.`3) = map (BytesToBits \o NBytes.val) (AuthPath.val auth{2}))
+           /\ DigestBlock.val cm{1} = BytesToBits (NBytes.val _M'{2})
+           /\ address{2} = zero_address
+           /\ DigestBlock.val pk{1}.`1 = BytesToBits (NBytes.val root{2})
+           /\ pk{1}.`2 = _seed{2}
+           /\ root{2} = pk{2}.`pk_root).
++ auto => &1 &2 /> eqpk11 eqpk12 eqsig11 eqsig12 eqsig21 ?? eqsig22 eqsig23 ltl_sig.
+  do ! split.
+(*   + rewrite eqsig21 Index.insubdK 2://.
+    smt(W32.to_uint_cmp). *)
+  + rewrite eqsig22 DBLL.insubdK.
+    + admit.x
+    rewrite -map_comp /=.
+    apply eq_map => x @/(\o).
+    apply DigestBlock.insubdK.
+    admit.
+  + rewrite eqsig23 DBHL.insubdK. admit.
+    rewrite -map_comp /=.
+    apply eq_map => x @/(\o).
+    apply DigestBlock.insubdK.
+    admit.
+  + rewrite /bs2block.
+    rewrite DigestBlock.insubdK.
+    admit.
+    do 4! congr.
+    rewrite eqsig11 eqsig12.
+    congr; 1: congr.
+    admit.
+    rewrite to_uintK NBytes.insubdK.
+    admit.
+    admit (* n = 4? *).
+  rewrite eqpk11.
+  rewrite DigestBlock.insubdK //.
+  admit.
+inline{1} verify; inline{2} rootFromSig.
+wp.
+swap{1} ^pk1<- @^pk0<- & +1.
+swap{1} ^root<- @^pk1<- & +1.
+sp 3 0.
+conseq (_: _ ==> DigestBlock.val root'{1} = BytesToBits (NBytes.val nodes0{2})).
++ move=> /> &1 &2 eqpk1 eqpk2 ltlsig eqsigfl1 eqsigfl2 eqsigfl3 eqcm eqvpk1.
+  move=> r0 r1 eqrs.
+  rewrite -DigestBlock.valKd eqrs eqpk1.
+  admit.
+  
+inline{1} root_from_sigFLXMSSTW.
+seq 14 11 : (   to_uint idx_sig0{2} < l
+             /\ ps0{1} = _seed0{2}
+             /\ map DigestBlock.val (DBLL.val pkWOTS0{1}) =  map (BytesToBits \o NBytes.val) (LenNBytes.val pk_ots{2})
+             /\ (set_kpidx (set_typeidx ad0{1} pkcotype) (Index.val idx{1})) = address0{2}
+             /\ Index.val idx{1} = to_uint idx_sig0{2}
+             /\ (DBHL.val ap{1}) = map bs2block (AuthPath.val auth0{2})).
++ admit.
+seq 1 3 : (   to_uint idx_sig0{2} < l
+           /\ ps0{1} = _seed0{2}
+           /\ (set_thtbidx (set_typeidx ad0{1} trhtype) 0 (Index.val idx{1})) = address0{2}
+           /\ Index.val idx{1} = to_uint idx_sig0{2}
+           /\ leaf{1} = bs2block nodes0{2}
+           /\ (DBHL.val ap{1}) = map bs2block (AuthPath.val auth0{2})).
+wp.
+have ltree_ll : islossless LTree.ltree by admit.
+exlim pk_ots{2}, address0{2}, _seed0{2} => pkots2 add02 sd02. 
+call{2} (_: arg = (pkots2, add02, sd02) ==> res = ltree  sd02 add02 pkots2).  print Eqv_Ltree_ltree.
+by conseq ltree_ll (ltree_eq sd02 add02 pkots2).
+skip => &1 &2 /> ltlidx eqpkots eqidx eqap.
+split.
+rewrite /trhtype. (* instantiate addresses so that setting entries can be matched...*)
+admit.
+rewrite /pkco /thfc /=.
+rewrite (: 8 * n * XMSS_ABSTRACT.FLXMSSTW.len <> 8 * n). admit.
+rewrite (: 8 * n * XMSS_ABSTRACT.FLXMSSTW.len <> 8 * n * 2) /=. admit. (* requires len <> 2... *)
+rewrite /bs2block /pkcotype. do 4! congr.
+rewrite eqpkots. admit.
+
+exlim nodes0{2}, address0{2} => lf2 ad2.
+while{2} (BytesToBits (NBytes.val nodes0{2})
+          =
+          (let app = drop (h - k{2}) (map bs2block (AuthPath.val auth0{2})) in
+           let idp = (rev (BS2Int.int2bs k{2} (to_uint idx_sig0{2}))) in
+           let lfp = bs2block lf2 in
+           DigestBlock.val (val_ap_trh_gen app idp lfp _seed0{2} ad2 k{2} (to_uint idx_sig0{2} %/ 2 ^ k{2})))
+          /\ 0 <= k{2} <= h)
+         (h - k{2}).
++ move=> _ z.
+  wp.
+  proc change 2 : (! odd (to_uint idx_sig0 %/ 2 ^ k)).
+  + admit.
+  sp.
+  have rand_hash_ll : islossless Hash.rand_hash by admit.
+  if => //.
+  + sp.
+    exlim nodes0, auth_k, _seed0, address0 => nds0 apk sd0 ad0.
+    call (_: arg = (nds0, apk, sd0, ad0) ==> res = rand_hash nds0 apk sd0 ad0).
+    by conseq rand_hash_ll (rand_hash_eq nds0 apk sd0 ad0).
+  skip => &1 /> ad01 ih ge0_k _ lth_k cut_even.
+  rewrite -!andbA; split => [| /#].
+  rewrite (: h - (k{1} + 1) = h - k{1} - 1) 1:/#.
+  rewrite (drop_nth witness) 1:size_map 1:AuthPath.valP 1:/# /=.
+  rewrite BS2Int.int2bsS 1:// rev_rcons /=.
+  rewrite (: to_uint idx_sig0{1} %/ 2 ^ k{1} %% 2 = 0) /=. smt(oddP).
+  rewrite (: 2 * (to_uint idx_sig0{1} %/ 2 ^ (k{1} + 1)) = (to_uint idx_sig0{1} %/ 2 ^ k{1})). admit.
+  rewrite -ih /trh /thfc (: 8 * n * 2 <> 8 * n) /=; 1: smt(ge1_n).
+  rewrite /rand_hash /=. admit.
+  + sp.
+    exlim auth_k, nodes0, _seed0, address0 => apk nds0 sd0 ad0.
+    call (_: arg = (apk, nds0, sd0, ad0) ==> res = rand_hash apk nds0 sd0 ad0).
+    by conseq rand_hash_ll (rand_hash_eq apk nds0 sd0 ad0).
+  skip => &1 /> ad01 ih ge0_k _ lth_k cut_even.
+  rewrite -!andbA; split => [| /#].
+  rewrite (: h - (k{1} + 1) = h - k{1} - 1) 1:/#.
+  rewrite (drop_nth witness) 1:size_map 1:AuthPath.valP 1:/# /=.
+  rewrite BS2Int.int2bsS 1:// rev_rcons /=.
+  rewrite (: to_uint idx_sig0{1} %/ 2 ^ k{1} %% 2 <> 0) /=. smt(oddP).
+  rewrite (: 2 * (to_uint idx_sig0{1} %/ 2 ^ (k{1} + 1)) + 1 = (to_uint idx_sig0{1} %/ 2 ^ k{1})). admit.
+  rewrite -ih /trh /thfc (: 8 * n * 2 <> 8 * n) /=; 1: smt(ge1_n).
+  rewrite /rand_hash /=. admit.
+wp; skip => &1 &2 /> ltlidx eqidx eqap.
+split.
+rewrite BS2Int.int2bs0s rev_nil /val_ap_trh_gen -eqap.
+rewrite (: h = size (DBHL.val ap{1})) 1:DBHL.valP 1:// drop_size /=.
+rewrite /bs2block DigestBlock.insubdK 2://. admit.
+move => kr nds0.
+split => [/# | /lezNgt geh_kr -> ge0_kr leh_kr].
+rewrite (: kr = h) 1:/#.
+rewrite /val_ap_trh /= drop0 eqap eqidx.
+rewrite (: (to_uint idx_sig0{2} %/ 2 ^ h) = 0).
+rewrite -divz_eq0 1:IntOrder.expr_gt0 1://; smt(W32.to_uint_cmp).
+have: valid_tbidx 0 (to_uint idx_sig0{2}). admit.
+move: (to_uint idx_sig0{2}) => i valtb.
+congr.
+admit. (* Annoying, but true: th and tb idx is always overwritten *)
+qed.
+*)
